Change the normalisation for extraction
- Normalise only the structure but let the extraction of F* unfold the
  implementations in Steel
- Allow hiding the Steel parts in .fst

experiment/Experiment.Steel.Combinators.fst
@@ -1,40 +1,18 @@
 module Experiment.Steel.Combinators
 
-module U   = Learn.Util
 module L   = FStar.List.Pure
-module T   = FStar.Tactics
-module SE  = Steel.Effect
-module SH  = Experiment.Steel.Steel
-module Fl  = Learn.FList
-module Mem = Steel.Memory
-module Veq = Experiment.Steel.VEquiv
-module TcS = Experiment.Steel.Tac
 
-open Steel.Effect
-open Steel.Effect.Atomic
-open Experiment.Steel.Interface
-open Experiment.Steel.VPropList
-open Experiment.Steel.Repr.M
-
-#push-options "--ifuel 1 --ide_id_info_off"
-
-/// We define a "monad" (which does not satisfy the monad laws) on [M.repr]. 
-
-unfold
-let repr_steel_tc
-      (ek : SH.effect_kind) (#a : Type) (#t : prog_tree a) (#pre : pre_t) (#post : post_t a)
-      ($tc : tree_cond t pre post)
-  : Type
-  = repr_steel_t ek a pre post (tree_req t tc) (tree_ens t tc)
+#set-options "--ifuel 1 --ide_id_info_off"
 
 (****** Call *)
 
 #push-options "--z3rlimit 30"
 inline_for_extraction noextract
 let tcspec_steel__steel
-      (a : Type) (pre : pre_t) (post : post_t a) (ro : vprop_list)
-      (req : sl_f pre -> sl_f ro -> Type0) (ens : sl_f pre -> (x : a) -> sl_f (post x) -> sl_f ro -> Type0)
-      (tcs : tree_cond_Spec a L.(pre @ ro) (spc_post1 (Mkspec_r pre post ro req ens)))
+      (a : Type)
+      (pre : G.erased pre_t) (post : G.erased (post_t a)) (ro : G.erased vprop_list)
+      (req : sl_f pre -> sl_f ro -> Type0) (ens : sl_f pre -> (x : a) -> sl_f (G.reveal post x) -> sl_f ro -> Type0)
+      (tcs : G.erased (tree_cond_Spec a L.(pre @ ro) (spc_post1 (Mkspec_r pre post ro req ens))))
       ($f : spc_steel_t SH.KSteel (Mkspec_r pre post ro req ens))
   : repr_steel_tc SH.KSteel (TCspec #a #(spec_r_exact (Mkspec_r pre post ro req ens)) _ SpecExact tcs)
   = SH.steel_f (fun () ->
@@ -42,16 +20,17 @@ let tcspec_steel__steel
     (**) elim_vpl_append L.(pre @ ro) tcs.tcs_frame;
     (**) elim_vpl_append pre ro;
     let (x : a) = SH.steel_c f () in
-    (**) intro_vpl_append (post x) ro;
-    (**) intro_vpl_append L.(post x @ ro) tcs.tcs_frame;
+    (**) intro_vpl_append (G.reveal post x) ro;
+    (**) intro_vpl_append L.(G.reveal post x @ ro) tcs.tcs_frame;
     (**) (tcs.tcs_post_eq x).veq_g _;
     Steel.Effect.Atomic.return x)
 
 inline_for_extraction noextract
 let tcspec_steel__atomic
-      (a : Type) (opened : Mem.inames) (pre : pre_t) (post : post_t a) (ro : vprop_list)
-      (req : sl_f pre -> sl_f ro -> Type0) (ens : sl_f pre -> (x : a) -> sl_f (post x) -> sl_f ro -> Type0)
-      (tcs : tree_cond_Spec a L.(pre @ ro) (spc_post1 (Mkspec_r pre post ro req ens)))
+      (a : Type) (opened : Mem.inames)
+      (pre : G.erased pre_t) (post : G.erased (post_t a)) (ro : G.erased vprop_list)
+      (req : sl_f pre -> sl_f ro -> Type0) (ens : sl_f pre -> (x : a) -> sl_f (G.reveal post x) -> sl_f ro -> Type0)
+      (tcs : G.erased (tree_cond_Spec a L.(pre @ ro) (spc_post1 (Mkspec_r pre post ro req ens))))
       ($f : spc_steel_t (SH.KAtomic opened) (Mkspec_r pre post ro req ens))
   : repr_steel_tc (SH.KAtomic opened) (TCspec #a #(spec_r_exact (Mkspec_r pre post ro req ens)) _ SpecExact tcs)
   = SH.atomic_f #opened (fun () ->
@@ -59,16 +38,17 @@ let tcspec_steel__atomic
     (**) elim_vpl_append L.(pre @ ro) tcs.tcs_frame;
     (**) elim_vpl_append pre ro;
     let (x : a) = SH.atomic_c f () in
-    (**) intro_vpl_append (post x) ro;
-    (**) intro_vpl_append L.(post x @ ro) tcs.tcs_frame;
+    (**) intro_vpl_append (G.reveal post x) ro;
+    (**) intro_vpl_append L.(G.reveal post x @ ro) tcs.tcs_frame;
     (**) (tcs.tcs_post_eq x).veq_g _;
     Steel.Effect.Atomic.return x)
 
 inline_for_extraction noextract
 let tcspec_steel__ghostI
-      (a : Type) (opened : Mem.inames) (pre : pre_t) (post : post_t a) (ro : vprop_list)
-      (req : sl_f pre -> sl_f ro -> Type0) (ens : sl_f pre -> (x : a) -> sl_f (post x) -> sl_f ro -> Type0)
-      (tcs : tree_cond_Spec a L.(pre @ ro) (spc_post1 (Mkspec_r pre post ro req ens)))
+      (a : Type) (opened : Mem.inames)
+      (pre : G.erased pre_t) (post : G.erased (post_t a)) (ro : G.erased vprop_list)
+      (req : sl_f pre -> sl_f ro -> Type0) (ens : sl_f pre -> (x : a) -> sl_f (G.reveal post x) -> sl_f ro -> Type0)
+      (tcs : G.erased (tree_cond_Spec a L.(pre @ ro) (spc_post1 (Mkspec_r pre post ro req ens))))
       ($f : spc_steel_t (SH.KGhostI opened) (Mkspec_r pre post ro req ens))
   : repr_steel_tc (SH.KGhostI opened) (TCspec #a #(spec_r_exact (Mkspec_r pre post ro req ens)) _ SpecExact tcs)
   = SH.ghostI_f #opened (fun () ->
@@ -76,16 +56,17 @@ let tcspec_steel__ghostI
     (**) elim_vpl_append L.(pre @ ro) tcs.tcs_frame;
     (**) elim_vpl_append pre ro;
     let (x : a) = SH.ghostI_c f () in
-    (**) intro_vpl_append (post x) ro;
-    (**) intro_vpl_append L.(post x @ ro) tcs.tcs_frame;
+    (**) intro_vpl_append (G.reveal post x) ro;
+    (**) intro_vpl_append L.(G.reveal post x @ ro) tcs.tcs_frame;
     (**) (tcs.tcs_post_eq x).veq_g _;
     Steel.Effect.Atomic.return x)
 
 inline_for_extraction noextract
 let tcspec_steel__ghost
-      (a : Type) (opened : Mem.inames) (pre : pre_t) (post : post_t a) (ro : vprop_list)
-      (req : sl_f pre -> sl_f ro -> Type0) (ens : sl_f pre -> (x : a) -> sl_f (post x) -> sl_f ro -> Type0)
-      (tcs : tree_cond_Spec a L.(pre @ ro) (spc_post1 (Mkspec_r pre post ro req ens)))
+      (a : Type) (opened : Mem.inames)
+      (pre : G.erased pre_t) (post : G.erased (post_t a)) (ro : G.erased vprop_list)
+      (req : sl_f pre -> sl_f ro -> Type0) (ens : sl_f pre -> (x : a) -> sl_f (G.reveal post x) -> sl_f ro -> Type0)
+      (tcs : G.erased (tree_cond_Spec a L.(pre @ ro) (spc_post1 (Mkspec_r pre post ro req ens))))
       ($f : spc_steel_t (SH.KGhost opened) (Mkspec_r pre post ro req ens))
   : repr_steel_tc (SH.KGhost opened) (TCspec #a #(spec_r_exact (Mkspec_r pre post ro req ens)) _ SpecExact tcs)
   = SH.ghost_f #opened (fun () ->
@@ -93,8 +74,8 @@ let tcspec_steel__ghost
     (**) elim_vpl_append L.(pre @ ro) tcs.tcs_frame;
     (**) elim_vpl_append pre ro;
     let (x : a) = SH.ghost_c f () in
-    (**) intro_vpl_append (post x) ro;
-    (**) intro_vpl_append L.(post x @ ro) tcs.tcs_frame;
+    (**) intro_vpl_append (G.reveal post x) ro;
+    (**) intro_vpl_append L.(G.reveal post x @ ro) tcs.tcs_frame;
     (**) (tcs.tcs_post_eq x).veq_g _;
     (**) noop ();
     x)
@@ -102,9 +83,10 @@ let tcspec_steel__ghost
 
 inline_for_extraction noextract
 let tcspec_steel
-      (a : Type) (ek : SH.effect_kind) (pre : pre_t) (post : post_t a) (ro : vprop_list)
-      (req : sl_f pre -> sl_f ro -> Type0) (ens : sl_f pre -> (x : a) -> sl_f (post x) -> sl_f ro -> Type0)
-      (tcs : tree_cond_Spec a L.(pre @ ro) (spc_post1 (Mkspec_r pre post ro req ens)))
+      (a : Type) (ek : SH.effect_kind)
+      (pre : G.erased pre_t) (post : G.erased (post_t a)) (ro : G.erased vprop_list)
+      (req : sl_f pre -> sl_f ro -> Type0) (ens : sl_f pre -> (x : a) -> sl_f (G.reveal post x) -> sl_f ro -> Type0)
+      (tcs : G.erased (tree_cond_Spec a L.(pre @ ro) (spc_post1 (Mkspec_r pre post ro req ens))))
       ($f : spc_steel_t ek (Mkspec_r pre post ro req ens))
   : repr_steel_tc ek (TCspec #a #(spec_r_exact (Mkspec_r pre post ro req ens)) _ SpecExact tcs)
   = match ek with
@@ -113,68 +95,13 @@ let tcspec_steel
   | SH.KGhostI o -> tcspec_steel__ghostI a o pre post ro req ens tcs f
   | SH.KGhost  o -> tcspec_steel__ghost  a o pre post ro req ens tcs f
 
-
-[@@ __repr_M__]
-let tree_of_steel_r (#ek : SH.effect_kind) (#a : Type) (#s : spec_r a) ($f : spc_steel_t ek s)
-  : prog_tree a
-  = Tspec a (spec_r_exact s)
-
-[@@ __repr_M__]
-inline_for_extraction noextract
-let repr_of_steel_r
-      (#a : Type) (s : spec_r a) (#ek : SH.effect_kind) ($f : spc_steel_t ek s)
-  : repr ek a
-  = {
-    repr_tree  = tree_of_steel_r f;
-    repr_steel = (fun pre'0 post'0 c ->
-                    let TCspec _ _ tcs = c in
-                    let Mkspec_r pre0 post0 ro0 req0 ens0 = s in
-                    tcspec_steel a ek pre0 post0 ro0 req0 ens0 tcs f)
-  }
-
-
-[@@ __repr_M__]
-let tree_of_steel
-      (#a : Type) (#pre : SE.pre_t) (#post : SE.post_t a) (#req : SE.req_t pre) (#ens : SE.ens_t pre a post)
-      (#ek : SH.effect_kind) ($f : SH.steel a pre post req ens ek)
-  : prog_tree a
-  = Tspec a (spec_r_steel pre post req ens)
-
-// FIXME? delta_only & delta_attr do not work under a match, but delta_qualifier does
-private
-let __postprocess_steps : list norm_step = [
-  delta_qualifier ["inline_for_extraction"];
-  iota
-]
-
-//[@@ __repr_M__; FStar.Tactics.(postprocess_with (fun () -> norm __postprocess_steps; trefl ()))]
-[@@ __repr_M__]
-inline_for_extraction noextract
-let repr_of_steel
-      (#a : Type) (pre : SE.pre_t) (post : SE.post_t a) (req : SE.req_t pre) (ens : SE.ens_t pre a post)
-      (#ek : SH.effect_kind) ($f : SH.steel a pre post req ens ek)
-  : repr ek a
-  = {
-    repr_tree  = tree_of_steel f;
-    repr_steel = (fun pre'0 post'0 c ->
-                    let TCspec #a #sp s sh tcs = c in
-                    let SpecSteel tr (Mkspec_find_ro (Mkspec_r pre0 post0 ro0 req0 ens0)
-                                                     pre_eq post_eq req_eq ens_eq)
-                      = U.cast (spec_r_steel pre post req ens s) sh in
-                    let sr = Mkspec_find_ro (Mkspec_r pre0 post0 ro0 req0 ens0)
-                                            pre_eq post_eq req_eq ens_eq in
-                    tcspec_steel a ek pre0 post0 ro0 req0 ens0 tcs
-                       (spec_r_of_find_ro sr (repr_of_steel tr f)))
-  }
-
-
 (****** Return *)
 
 inline_for_extraction noextract
 let return_steel__steel
       (a : Type) (x : a) (sl_hint : option (post_t a))
-      (pre : pre_t) (post : post_t a)
-      (e : Veq.vequiv pre (post x))
+      (pre : G.erased pre_t) (post : G.erased (post_t a))
+      (e : Veq.vequiv pre (G.reveal post x))
   : repr_steel_tc SH.KSteel (TCret #a #x #sl_hint pre post e)
   = SH.steel_f (fun () ->
     (**) e.veq_g _;
@@ -183,8 +110,8 @@ let return_steel__steel
 inline_for_extraction noextract
 let return_steel__atomic
       (a : Type) (opened : Mem.inames) (x : a) (sl_hint : option (post_t a))
-      (pre : pre_t) (post : post_t a)
-      (e : Veq.vequiv pre (post x))
+      (pre : G.erased pre_t) (post : G.erased (post_t a))
+      (e : Veq.vequiv pre (G.reveal post x))
   : repr_steel_tc (SH.KAtomic opened) (TCret #a #x #sl_hint pre post e)
   = SH.atomic_f #opened (fun () ->
     (**) e.veq_g _;
@@ -193,8 +120,8 @@ let return_steel__atomic
 inline_for_extraction noextract
 let return_steel__ghostI
       (a : Type) (opened : Mem.inames) (x : a) (sl_hint : option (post_t a))
-      (pre : pre_t) (post : post_t a)
-      (e : Veq.vequiv pre (post x))
+      (pre : G.erased pre_t) (post : G.erased (post_t a))
+      (e : Veq.vequiv pre (G.reveal post x))
   : repr_steel_tc (SH.KGhostI opened) (TCret #a #x #sl_hint pre post e)
   = SH.ghostI_f #opened (fun () ->
     (**) e.veq_g _;
@@ -203,8 +130,8 @@ let return_steel__ghostI
 inline_for_extraction noextract
 let return_steel__ghost
       (a : Type) (opened : Mem.inames) (x : a) (sl_hint : option (post_t a))
-      (pre : pre_t) (post : post_t a)
-      (e : Veq.vequiv pre (post x))
+      (pre : G.erased pre_t) (post : G.erased (post_t a))
+      (e : Veq.vequiv pre (G.reveal post x))
   : repr_steel_tc (SH.KGhost opened) (TCret #a #x #sl_hint pre post e)
   = SH.ghost_f #opened (fun () ->
     (**) e.veq_g _;
@@ -213,32 +140,14 @@ let return_steel__ghost
 inline_for_extraction noextract
 let return_steel
       (a : Type) (ek : SH.effect_kind) (x : a) (sl_hint : option (post_t a))
-      (pre : pre_t) (post : post_t a)
-      (e : Veq.vequiv pre (post x))
+      (pre : G.erased pre_t) (post : G.erased (post_t a))
+      (e : Veq.vequiv pre (G.reveal post x))
   : repr_steel_tc ek (TCret #a #x #sl_hint pre post e)
   = match ek with
   | SH.KSteel    -> return_steel__steel  a   x sl_hint pre post e
   | SH.KAtomic o -> return_steel__atomic a o x sl_hint pre post e
   | SH.KGhostI o -> return_steel__ghostI a o x sl_hint pre post e
   | SH.KGhost  o -> return_steel__ghost  a o x sl_hint pre post e
-
-
-[@@ __repr_M__]
-inline_for_extraction noextract
-let return_hint (ek : SH.effect_kind) (#a : Type) (x : a) (sl_hint : option (post_t a))
-  : repr ek a
-  = {
-    repr_tree  = Tret a x sl_hint;
-    repr_steel = (fun pre0 post0 c ->
-        let TCret pre post p = c in
-        return_steel a ek x sl_hint pre post p)
-  }
-
-[@@ __repr_M__]
-inline_for_extraction noextract
-let return (ek : SH.effect_kind) (#a : Type) (x : a) : repr ek a
-  = return_hint ek x None
-
 
 (****** Bind *)
 
@@ -271,467 +180,186 @@ let intro_tree_ens_bind (#a #b : Type) (f : prog_tree a) (g : a -> prog_tree b)
           tree_ens (g x) (cg x) sl1 y sl2)
     ))
 
-[@@FStar.Tactics.(postprocess_with (fun () -> norm __postprocess_steps; trefl ()))]
+#push-options "--ifuel 0 --fuel 0 --z3rlimit 20"
 inline_for_extraction noextract
-let bind_steel
-      (a : Type) (b : Type) (f : prog_tree a) (g : (a -> prog_tree b))
-      (pre : pre_t) (itm : post_t a) (post : post_t b)
-      (cf : tree_cond f pre itm) (cg : ((x : a) -> tree_cond (g x) (itm x) post))
-      ($rf : repr_steel_t SH.KSteel a pre itm (tree_req f cf) (tree_ens f cf))
-      ($rg : (x : a) -> repr_steel_t SH.KSteel b (itm x) post (tree_req (g x) (cg x)) (tree_ens (g x) (cg x)))
-  : repr_steel_tc SH.KSteel (TCbind #a #b #f #g pre itm post cf cg)
+let bind_steel__steel a b f g pre itm post cf cg rf rg
   = SH.steel_f (fun () ->
     (**) let sl0 = gget (vprop_of_list pre) in
     (**) (elim_tree_req_bind f g cf cg sl0; ());
     let x = SH.steel_u rf () in
-    (**) let sl1 = gget (vprop_of_list (itm x)) in
+    (**) let sl1 = gget (vprop_of_list (G.reveal itm x)) in
     let y = SH.steel_u (rg x) () in
-    (**) let sl2 = gget (vprop_of_list (post y)) in
+    (**) let sl2 = gget (vprop_of_list (G.reveal post y)) in
     (**) (intro_tree_ens_bind f g cf cg sl0 x sl1 y sl2; ());
     Steel.Effect.Atomic.return y)
 
-[@@FStar.Tactics.(postprocess_with (fun () -> norm __postprocess_steps; trefl ()))]
 inline_for_extraction noextract
-let bind_atomic_ghost_steel
-      (a : Type) (b : Type) (opened : Mem.inames) (f : prog_tree a) (g : (a -> prog_tree b))
-      (pre : pre_t) (itm : post_t a) (post : post_t b)
-      (cf : tree_cond f pre itm) (cg : ((x : a) -> tree_cond (g x) (itm x) post))
-      ($rf : repr_steel_t (SH.KAtomic opened) a pre itm (tree_req f cf) (tree_ens f cf))
-      ($rg : (x : a) ->
-             repr_steel_t (SH.KGhostI opened) b (itm x) post (tree_req (g x) (cg x)) (tree_ens (g x) (cg x)))
-  : repr_steel_tc (SH.KAtomic opened) (TCbind #a #b #f #g pre itm post cf cg)
+let bind_steel__atomic_ghost o a b f g pre itm post cf cg rf rg
   = SH.atomic_f (fun () ->
     (**) let sl0 = gget (vprop_of_list pre) in
     (**) (elim_tree_req_bind f g cf cg sl0; ());
     let x = SH.atomic_u rf () in
-    (**) let sl1 = gget (vprop_of_list (itm x)) in
+    (**) let sl1 = gget (vprop_of_list (G.reveal itm x)) in
     let y = SH.ghostI_u (rg x) () in
-    (**) let sl2 = gget (vprop_of_list (post y)) in
+    (**) let sl2 = gget (vprop_of_list (G.reveal post y)) in
     (**) (intro_tree_ens_bind f g cf cg sl0 x sl1 y sl2; ());
     Steel.Effect.Atomic.return y)
 
-[@@FStar.Tactics.(postprocess_with (fun () -> norm __postprocess_steps; trefl ()))]
 inline_for_extraction noextract
-let bind_ghost_atomic_steel
-      (a : Type) (b : Type) (opened : Mem.inames) (f : prog_tree a) (g : (a -> prog_tree b))
-      (pre : pre_t) (itm : post_t a) (post : post_t b)
-      (cf : tree_cond f pre itm) (cg : ((x : a) -> tree_cond (g x) (itm x) post))
-      ($rf : repr_steel_t (SH.KGhostI opened) a pre itm (tree_req f cf) (tree_ens f cf))
-      ($rg : (x : a) ->
-             repr_steel_t (SH.KAtomic opened) b (itm x) post (tree_req (g x) (cg x)) (tree_ens (g x) (cg x)))
-  : repr_steel_tc (SH.KAtomic opened) (TCbind #a #b #f #g pre itm post cf cg)
+let bind_steel__ghost_atomic o a b f g pre itm post cf cg rf rg
   = SH.atomic_f (fun () ->
     (**) let sl0 = gget (vprop_of_list pre) in
     (**) (elim_tree_req_bind f g cf cg sl0; ());
     let x = SH.ghostI_u rf () in
-    (**) let sl1 = gget (vprop_of_list (itm x)) in
+    (**) let sl1 = gget (vprop_of_list (G.reveal itm x)) in
     let y = SH.atomic_u (rg x) () in
-    (**) let sl2 = gget (vprop_of_list (post y)) in
+    (**) let sl2 = gget (vprop_of_list (G.reveal post y)) in
     (**) (intro_tree_ens_bind f g cf cg sl0 x sl1 y sl2; ());
     Steel.Effect.Atomic.return y)
 
-[@@FStar.Tactics.(postprocess_with (fun () -> norm __postprocess_steps; trefl ()))]
 inline_for_extraction noextract
-let bind_ghostI_steel
-      (a : Type) (b : Type) (opened : Mem.inames) (f : prog_tree a) (g : (a -> prog_tree b))
-      (pre : pre_t) (itm : post_t a) (post : post_t b)
-      (cf : tree_cond f pre itm) (cg : ((x : a) -> tree_cond (g x) (itm x) post))
-      ($rf : repr_steel_t (SH.KGhostI opened) a pre itm (tree_req f cf) (tree_ens f cf))
-      ($rg : (x : a) ->
-             repr_steel_t (SH.KGhostI opened) b (itm x) post (tree_req (g x) (cg x)) (tree_ens (g x) (cg x)))
-  : repr_steel_tc (SH.KGhostI opened) (TCbind #a #b #f #g pre itm post cf cg)
-  = SH.ghostI_f #opened (fun () ->
+let bind_steel__ghostI o a b f g pre itm post cf cg rf rg
+  = SH.ghostI_f (fun () ->
     (**) let sl0 = gget (vprop_of_list pre) in
     (**) (elim_tree_req_bind f g cf cg sl0; ());
     let x = SH.ghostI_u rf () in
-    (**) let sl1 = gget (vprop_of_list (itm x)) in
+    (**) let sl1 = gget (vprop_of_list (G.reveal itm x)) in
     let y = SH.ghostI_u (rg x) () in
-    (**) let sl2 = gget (vprop_of_list (post y)) in
+    (**) let sl2 = gget (vprop_of_list (G.reveal post y)) in
     (**) (intro_tree_ens_bind f g cf cg sl0 x sl1 y sl2; ());
     Steel.Effect.Atomic.return y)
 
-[@@FStar.Tactics.(postprocess_with (fun () -> norm __postprocess_steps; trefl ()))]
 inline_for_extraction noextract
-let bind_ghost_steel
-      (a : Type) (b : Type) (opened : Mem.inames) (f : prog_tree a) (g : (a -> prog_tree b))
-      (pre : pre_t) (itm : post_t a) (post : post_t b)
-      (cf : tree_cond f pre itm) (cg : ((x : a) -> tree_cond (g x) (itm x) post))
-      ($rf : repr_steel_t (SH.KGhost opened) a pre itm (tree_req f cf) (tree_ens f cf))
-      ($rg : (x : a) ->
-             repr_steel_t (SH.KGhost opened) b (itm x) post (tree_req (g x) (cg x)) (tree_ens (g x) (cg x)))
-  : repr_steel_tc (SH.KGhost opened) (TCbind #a #b #f #g pre itm post cf cg)
-  = SH.ghost_f #opened (fun () ->
+let bind_steel__ghost o a b f g pre itm post cf cg rf rg
+  = SH.ghost_f (fun () ->
     (**) let sl0 = gget (vprop_of_list pre) in
     (**) (elim_tree_req_bind f g cf cg sl0; ());
     let x = SH.ghost_u rf () in
-    (**) let sl1 = gget (vprop_of_list (itm x)) in
+    (**) let sl1 = gget (vprop_of_list (G.reveal itm x)) in
     let y = SH.ghost_u (rg x) () in
-    (**) let sl2 = gget (vprop_of_list (post y)) in
+    (**) let sl2 = gget (vprop_of_list (G.reveal post y)) in
     (**) (intro_tree_ens_bind f g cf cg sl0 x sl1 y sl2; ());
     (**) noop ();
     y)
+#pop-options
 
-
-[@@ __repr_M__]
-inline_for_extraction noextract
-let bind_ek (#a #b : Type) (ek0 ek1 ek2 : SH.effect_kind)
-      (s : (a : Type) -> (b : Type) -> (f : prog_tree a) -> (g : (a -> prog_tree b)) ->
-           (pre : pre_t) -> (itm : post_t a) -> (post : post_t b) ->
-           (cf : tree_cond f pre itm) -> (cg : ((x : a) -> tree_cond (g x) (itm x) post)) ->
-           (rf : repr_steel_t ek0 a pre itm (tree_req f cf) (tree_ens f cf)) ->
-           (rg : ((x : a) -> repr_steel_t ek1 b (itm x) post (tree_req (g x) (cg x)) (tree_ens (g x) (cg x)))) ->
-           (let c = TCbind #a #b #f #g pre itm post cf cg in
-            repr_steel_t ek2 b pre post (tree_req _ c) (tree_ens _ c)))
-      (f : repr ek0 a) (g : a -> repr ek1 b)
-  : repr ek2 b
-  = {
-    repr_tree  = Tbind a b f.repr_tree (fun x -> (g x).repr_tree);
-    repr_steel = (fun pre0 post0 c ->
-                    let (TCbind #a' #b' #tf #tg pre itm post cf cg) = c in
-                    let rg (x : a) : repr_steel_t ek1 b (itm x) post _ _
-                                   = (g x).repr_steel _ _ (cg x) in
-                    s a b tf tg pre itm post cf cg (f.repr_steel _ _ cf) rg)
-  }
-
-[@@ __repr_M__]
-inline_for_extraction noextract
-let bind (#a #b : Type) (f : repr SH.KSteel a) (g : a -> repr SH.KSteel b)
-  : repr SH.KSteel b
-  = bind_ek SH.KSteel SH.KSteel SH.KSteel
-      (fun a b f g pre itm post cf cg rf rg -> bind_steel a b f g pre itm post cf cg rf rg)
-      f g
-
-[@@ __repr_M__]
-inline_for_extraction noextract
-let bind_ghost (#a #b : Type) (#opened : Mem.inames)
-               (f : repr (SH.KGhost opened) a) (g : a -> repr (SH.KGhost opened) b)
-  : repr (SH.KGhost opened) b
-  = bind_ek (SH.KGhost opened) (SH.KGhost opened) (SH.KGhost opened)
-      (fun a b f g pre itm post cf cg rf rg -> bind_ghost_steel a b opened f g pre itm post cf cg rf rg)
-      f g
-
+(**) private let end_bind_steel = ()
 
 (****** Bind pure *)
 
+type bindP_steel_t (ek : SH.effect_kind) =
+      (a : Type) -> (b : Type) -> (wp : pure_wp a) -> (f : unit -> PURE a wp) ->
+      (g : G.erased (a -> prog_tree b)) ->
+      (pre : G.erased pre_t) -> (post : G.erased (post_t b)) ->
+      (cg : G.erased ((x : a) -> tree_cond (G.reveal g x) pre post)) ->
+      (rg : ((x : a) -> repr_steel_tc ek (G.reveal cg x))) ->
+      repr_steel_tc ek (TCbindP #a #b #wp #g pre post cg)
+
 inline_for_extraction noextract
-let bindP_steel__steel
-      (a : Type) (b : Type) (wp : pure_wp a) ($f : unit -> PURE a wp) (g : (a -> prog_tree b))
-      (pre : pre_t) (post : post_t b)
-      (cg : ((x : a) -> tree_cond (g x) pre post))
-      (rg : (x : a) -> repr_steel_t SH.KSteel b pre post (tree_req (g x) (cg x)) (tree_ens (g x) (cg x)))
-  : repr_steel_tc SH.KSteel (TCbindP #a #b #wp #g pre post cg)
-  = 
+let bindP_steel__steel : bindP_steel_t SH.KSteel
+  = fun a b wp f g pre post cg rg ->
     FStar.Monotonic.Pure.elim_pure_wp_monotonicity wp;
     SH.steel_f (fun () ->
     let x = f () in
     SH.steel_u (rg x) ())
 
 inline_for_extraction noextract
-let bindP_steel__atomic
-      (a : Type) (b : Type) (opened : Mem.inames) (wp : pure_wp a) ($f : unit -> PURE a wp) (g : (a -> prog_tree b))
-      (pre : pre_t) (post : post_t b)
-      (cg : ((x : a) -> tree_cond (g x) pre post))
-      (rg : (x : a) -> repr_steel_t (SH.KAtomic opened)  b pre post (tree_req (g x) (cg x)) (tree_ens (g x) (cg x)))
-  : repr_steel_tc (SH.KAtomic opened) (TCbindP #a #b #wp #g pre post cg)
-  = 
+let bindP_steel__atomic o : bindP_steel_t (SH.KAtomic o)
+  = fun a b wp f g pre post cg rg ->
     FStar.Monotonic.Pure.elim_pure_wp_monotonicity wp;
     SH.atomic_f (fun () ->
     let x = f () in
     SH.atomic_u (rg x) ())
 
 inline_for_extraction noextract
-let bindP_steel__ghostI
-      (a : Type) (b : Type) (opened : Mem.inames) (wp : pure_wp a) ($f : unit -> PURE a wp) (g : (a -> prog_tree b))
-      (pre : pre_t) (post : post_t b)
-      (cg : ((x : a) -> tree_cond (g x) pre post))
-      ($rg : (x : a) -> repr_steel_t (SH.KGhostI opened)  b pre post (tree_req (g x) (cg x)) (tree_ens (g x) (cg x)))
-  : repr_steel_tc (SH.KGhostI opened) (TCbindP #a #b #wp #g pre post cg)
-  = 
+let bindP_steel__ghostI o : bindP_steel_t (SH.KGhostI o)
+  = fun a b wp f g pre post cg rg ->
     FStar.Monotonic.Pure.elim_pure_wp_monotonicity wp;
     SH.ghostI_f (fun () ->
     let x = f () in
     SH.ghostI_u (rg x) ())
 
 inline_for_extraction noextract
-let bindP_steel__ghost0
-      (a : Type) (b : Type) (opened : Mem.inames) (wp : pure_wp a) ($f : unit -> PURE a wp) (g : (a -> prog_tree b))
-      (pre : pre_t) (post : post_t b)
-      (cg : ((x : a) -> tree_cond (g x) pre post))
-      (rg : (x : a) -> repr_steel_t (SH.KGhost opened) b pre post (tree_req (g x) (cg x)) (tree_ens (g x) (cg x)))
-  : repr_steel_tc (SH.KGhost opened) (TCbindP #a #b #wp #g pre post cg)
-  =
+let bindP_steel__ghost0 o : bindP_steel_t (SH.KGhost o)
+  = fun a b wp f g pre post cg rg ->
     FStar.Monotonic.Pure.elim_pure_wp_monotonicity wp;
-    SH.ghost_f #opened (fun () ->
+    SH.ghost_f (fun () ->
     let x = f () in
     SH.ghost_u (rg x) ())
 
 inline_for_extraction noextract
-let bindP_steel__ghost
-      (a : Type) (b : Type) (opened : Mem.inames) (wp : pure_wp a) ($f : unit -> GHOST a wp) (g : (a -> prog_tree b))
-      (pre : pre_t) (post : post_t b)
-      (cg : ((x : a) -> tree_cond (g x) pre post))
-      (rg : (x : a) -> repr_steel_t (SH.KGhost opened) b pre post (tree_req (g x) (cg x)) (tree_ens (g x) (cg x)))
-  : repr_steel_tc (SH.KGhost opened) (TCbindP #a #b #wp #g pre post cg)
+let bindP_steel__ghost a b o wp f g pre post cg rg
   =
     FStar.Monotonic.Pure.elim_pure_wp_monotonicity wp;
-    SH.ghost_f #opened (fun () ->
+    SH.ghost_f (fun () ->
     let x = f () in
     SH.ghost_u (rg x) ())
 
-#push-options "--ifuel 1 --fuel 1 --z3rlimit 10"
-[@@ __repr_M__]
 inline_for_extraction noextract
-let bindP (#a #b : Type) (ek : SH.effect_kind) (wp : pure_wp a) ($f : unit -> PURE a wp) (g : a -> repr ek b)
-  : repr ek b
-  = {
-    repr_tree  = TbindP a b wp (fun x -> (g x).repr_tree);
-    repr_steel = (fun pre0 post0 c ->
-                    let (TCbindP #a' #b' #wp #tg pre post cg) = c in
-                    let rg (x : a) : repr_steel_t ek b pre post _ _
-                                   = (g x).repr_steel _ _ (cg x) in
-                    match ek returns repr_steel_t ek b _ _ _ _ with
-                    | SH.KSteel    -> bindP_steel__steel  a b   wp f tg pre post cg rg
-                    | SH.KAtomic o -> bindP_steel__atomic a b o wp f tg pre post cg rg
-                    | SH.KGhostI o -> bindP_steel__ghostI a b o wp f tg pre post cg rg
-                    | SH.KGhost  o -> bindP_steel__ghost0 a b o wp f tg pre post cg rg
-                 )
-  }
-
-[@@ __repr_M__]
-inline_for_extraction noextract
-let bindP_ghost (#a #b : Type) (#opened : Mem.inames)
-                (wp : pure_wp a) ($f : unit -> GHOST a wp) (g : a -> repr (SH.KGhost opened) b)
-  : repr (SH.KGhost opened) b
-  = {
-    repr_tree  = TbindP a b wp (fun x -> (g x).repr_tree);
-    repr_steel = (fun pre0 post0 c ->
-                    let (TCbindP #a' #b' #wp #tg pre post cg) = c in
-                    let rg (x : a) : repr_steel_t (SH.KGhost opened) b pre post _ _
-                                   = (g x).repr_steel _ _ (cg x) in
-                    bindP_steel__ghost a b opened wp f tg pre post cg rg)
-  }
-
+let bindP_steel
+      (a : Type) (b : Type) (ek : SH.effect_kind) (wp : pure_wp a) ($f : unit -> PURE a wp)
+      (g : G.erased (a -> prog_tree b))
+      (pre : G.erased pre_t) (post : G.erased (post_t b))
+      (cg : ((x : a) -> tree_cond (G.reveal g x) pre post))
+      (rg : (x : a) -> repr_steel_tc ek (G.reveal cg x))
+  : repr_steel_tc ek (TCbindP #a #b #wp #g pre post cg)
+  = match ek with
+  | SH.KSteel    -> bindP_steel__steel    a b wp f g pre post cg rg
+  | SH.KAtomic o -> bindP_steel__atomic o a b wp f g pre post cg rg
+  | SH.KGhostI o -> bindP_steel__ghostI o a b wp f g pre post cg rg
+  | SH.KGhost  o -> bindP_steel__ghost0 o a b wp f g pre post cg rg
 
 (****** If-then-else *)
 
 inline_for_extraction noextract
-let ite_steel
-      (a : Type) (guard : bool) (thn : prog_tree a) (els : prog_tree a)
-      (pre : pre_t) (post : post_t a)
-      (cthn : tree_cond thn pre post) (cels : tree_cond els pre post)
-      ($rthn : repr_steel_t SH.KSteel a pre post (tree_req thn cthn) (tree_ens thn cthn))
-      ($rels : repr_steel_t SH.KSteel a pre post (tree_req els cels) (tree_ens els cels))
-  : repr_steel_tc SH.KSteel (TCif #a #guard #thn #els pre post cthn cels)
+let ite_steel a guard thn els pre post cthn cels rthn rels
   = SH.steel_f (fun () ->
     if guard then SH.steel_u rthn () else SH.steel_u rels ())
 
 inline_for_extraction noextract
-let ite_ghost_steel
-      (a : Type) (opened : Mem.inames) (guard : bool) (thn : prog_tree a) (els : prog_tree a)
-      (pre : pre_t) (post : post_t a)
-      (cthn : tree_cond thn pre post) (cels : tree_cond els pre post)
-      ($rthn : repr_steel_t (SH.KGhost opened) a pre post (tree_req thn cthn) (tree_ens thn cthn))
-      ($rels : repr_steel_t (SH.KGhost opened) a pre post (tree_req els cels) (tree_ens els cels))
-  : repr_steel_tc (SH.KGhost opened) (TCif #a #guard #thn #els pre post cthn cels)
-  = SH.ghost_f #opened (fun () ->
+let ite_ghost_steel a opened guard thn els pre post cthn cels rthn rels
+  = SH.ghost_f (fun () ->
     if guard then SH.ghost_u rthn () else SH.ghost_u rels ())
-
-
-[@@ __repr_M__]
-inline_for_extraction noextract
-let ite (#a : Type) (guard : bool) (thn els : repr SH.KSteel a)
-  : repr SH.KSteel a
-  = {
-    repr_tree  = Tif a guard thn.repr_tree els.repr_tree;
-    repr_steel = (fun pre0 post0 c ->
-                    let TCif pre post cthn cels = c in
-                    ite_steel a guard _ _ pre post cthn cels
-                       (thn.repr_steel _ _ cthn) (els.repr_steel _ _ cels))
-  }
-
-[@@ __repr_M__]
-inline_for_extraction noextract
-let ite_ghost (#a : Type) (#opened : Mem.inames) (guard : bool) (thn els : repr (SH.KGhost opened) a)
-  : repr (SH.KGhost opened) a
-  = {
-    repr_tree  = Tif a guard thn.repr_tree els.repr_tree;
-    repr_steel = (fun pre0 post0 c ->
-                    let (TCif pre post cthn cels) = c in
-                    ite_ghost_steel a opened guard _ _ pre post cthn cels
-                       (thn.repr_steel _ _ cthn) (els.repr_steel _ _ cels))
-  }
-
-
-
-(*** Lifts *)
-
-(***** [erasable_t] *)
-
-type revealed_value (#a : Type) (x : Ghost.erased a) =
-  x' : a { x' == Ghost.reveal x }
-
-noeq inline_for_extraction noextract
-type erasable_t (a : Type) = {
-  erasable_rv : (x : Ghost.erased a) -> revealed_value x
-}
-
-private
-let __build_revealed_value (a : Type) : (x : Ghost.erased a) -> GTot (revealed_value x)
-  = fun x -> Ghost.reveal x
-
-/// Solves a goal [erasable_t a] if a is an erasable type.
-let build_erasable_t fr ctx : T.Tac unit
-  = T.(
-    let a : term
-      = match inspect (cur_goal ()) with
-        | Tv_App  _ arg -> arg._1
-        | _ -> fail "build_erasable_t : goal"
-    in
-    apply (`Mkerasable_t);
-    // The following requires a conversion from [_ -> GTot (revealed_value x)] to [_ -> Tot (revealed_value x)]
-    // which succeeds iff [revealed_value x] (i.e. [a]) is erasable.
-    // Since we use (`#a), this may generate some guards to retypecheck (`#a).
-    with_policy SMT (fun () -> TcS.cs_try (fun () ->
-      exact (`(__build_revealed_value (`#a) <: _ -> Tot _)))
-    fr ctx (fun m -> fail (m (Fail_not_erasable a) [])))
-  )
-
-private
-let test_erasable_unit : erasable_t unit
-  = _ by (build_erasable_t default_flags TcS.dummy_ctx)
-
-private
-let test_erasable_unit' : erasable_t U.unit'
-  = _ by (build_erasable_t default_flags TcS.dummy_ctx)
-
-#push-options "--silent"
-[@@ expect_failure [228]]
-private
-let test_erasable_int : erasable_t int
-  = _ by (build_erasable_t default_flags TcS.dummy_ctx)
-#pop-options
-
-[@@ erasable]
-private noeq
-type test_guard_type (_ : squash (forall (n : nat) . n >= 0)) =
-
-private
-let test_erasable_guard : erasable_t (test_guard_type ())
-  = _ by (build_erasable_t default_flags TcS.dummy_ctx)
-
 
 (***** [steel_liftable] *)
 
-// named as in Coq
-noeq
-type clos_refl_trans_1n (#a : Type) (r : a -> a -> Type) (x : a) : a -> Type =
-  | Rt1n_refl  : clos_refl_trans_1n r x x
-  | Rt1n_trans : (y : a) -> (z : a) ->
-                 r x y -> clos_refl_trans_1n r y z -> clos_refl_trans_1n r x z
-
-noeq
-type steel_liftable1 (a : Type) : SH.effect_kind -> SH.effect_kind -> Type =
-  | Lift_ghost_ghostI  : erasable_t a -> (opened : Mem.inames) ->
-                         steel_liftable1 a (SH.KGhost     opened) (SH.KGhostI opened)
-  | Lift_ghostI_atomic : (opened : Mem.inames) ->
-                         steel_liftable1 a (SH.KGhostI    opened) (SH.KAtomic opened)
-  | Lift_atomic_steel  : steel_liftable1 a (SH.KAtomic Set.empty)  SH.KSteel
-
-type steel_liftable (a : Type) : SH.effect_kind -> SH.effect_kind -> Type
-  = clos_refl_trans_1n (steel_liftable1 a)
-
-
-/// We define the lift on [repr_steel_t] rather than on [SH.steel] because the latter option does not work
-/// with steel's tactic because of the abstract specifications.
-
 let repr_steel_lift_ghost_ghostI_aux
-      #a #pre #post #req #ens #opened (f : repr_steel_t (SH.KGhost opened) a pre post req ens)
+      (#a : Type) (#pre : G.erased pre_t) (#post : G.erased (post_t a))
+      #req #ens #opened (f : repr_steel_t (SH.KGhost opened) a pre post req ens)
   : SH.unit_steel_ghost (Ghost.erased a) opened
-      (vprop_of_list pre) (fun x -> vprop_of_list (post (Ghost.reveal x)))
+      (vprop_of_list pre) (fun x -> vprop_of_list (G.reveal post (Ghost.reveal x)))
       (fun h0 -> req (sel_f pre h0))
-      (fun h0 x h1 -> ens (sel_f pre h0) (Ghost.reveal x) (sel_f (post (Ghost.reveal x)) h1))
+      (fun h0 x h1 -> ens (sel_f pre h0) (Ghost.reveal x) (sel_f (G.reveal post (Ghost.reveal x)) h1))
   =
     fun () ->
       let x = SH.ghost_u f () in
       Ghost.hide x
 
 inline_for_extraction noextract
-let repr_steel_lift_ghost_ghostI
-      #a #pre #post #req #ens opened (e : erasable_t a) (f : repr_steel_t (SH.KGhost opened) a pre post req ens)
-  : repr_steel_t (SH.KGhostI opened) a pre post req ens
+let repr_steel_lift_ghost_ghostI a opened e pre post req ens f
   =
     SH.ghostI_f (fun () ->
       let x : Ghost.erased a = repr_steel_lift_ghost_ghostI_aux f () in
       let x' : a = e.erasable_rv x in
-      change_equal_slprop (vprop_of_list (post (Ghost.reveal x))) (vprop_of_list (post x'));
+      change_equal_slprop (vprop_of_list (G.reveal post (Ghost.reveal x))) (vprop_of_list (G.reveal post x'));
       Steel.Effect.Atomic.return x'
   )
 
 inline_for_extraction noextract
-let repr_steel_lift_ghostI_atomic
-      #a #pre #post #req #ens opened (f : repr_steel_t (SH.KGhostI opened) a pre post req ens)
-  : repr_steel_t (SH.KAtomic opened) a pre post req ens
+let repr_steel_lift_ghostI_atomic a opened pre post req ens f
   = SH.atomic_f (fun () -> SH.ghostI_u f ())
 
 inline_for_extraction noextract
-let repr_steel_lift_atomic_steel
-      #a #pre #post #req #ens (f : repr_steel_t (SH.KAtomic Set.empty) a pre post req ens)
-  : repr_steel_t SH.KSteel a pre post req ens
+let repr_steel_lift_atomic_steel a pre post req ens f
   = SH.steel_f (fun () -> SH.atomic_u f ())
-
-inline_for_extraction noextract
-let repr_steel_lift1
-      (#a : Type) (#pre : pre_t) (#post : post_t a) (#req : req_t pre) (#ens : ens_t pre a post)
-      (#ek0 #ek1 : SH.effect_kind) (l : steel_liftable1 a ek0 ek1)
-      (f : repr_steel_t ek0 a pre post req ens)
-  : repr_steel_t ek1 a pre post req ens
-  = match l with
-  | Lift_ghost_ghostI e o -> repr_steel_lift_ghost_ghostI  o e f
-  | Lift_ghostI_atomic  o -> repr_steel_lift_ghostI_atomic o   f
-  | Lift_atomic_steel     -> repr_steel_lift_atomic_steel      f
-
-inline_for_extraction noextract
-let rec repr_steel_lift
-      (#a : Type) (#pre : pre_t) (#post : post_t a) (#req : req_t pre) (#ens : ens_t pre a post)
-      (#ek0 #ek1 : SH.effect_kind) (l : steel_liftable a ek0 ek1)
-      (f : repr_steel_t ek0 a pre post req ens)
-  : Tot (repr_steel_t ek1 a pre post req ens) (decreases l)
-  = match l with
-  | Rt1n_refl -> f
-  | Rt1n_trans _ _ l0 l1 -> repr_steel_lift l1 (repr_steel_lift1 l0 f)
-
-[@@ __repr_M__]
-inline_for_extraction noextract
-let repr_lift
-      (#a : Type) (#ek0 #ek1 : SH.effect_kind) (l : steel_liftable a ek0 ek1) (r : repr ek0 a)
-  : repr ek1 a
-  = { r with repr_steel = (fun pre post c -> repr_steel_lift l (r.repr_steel pre post c)) }
-
 
 (****** SteelGhost to Steel (Monad) *)
 
 inline_for_extraction noextract
-let ghost_to_steel_steel (a : Type) (t : prog_tree (Ghost.erased a)) (pre : pre_t) (post : post_t (Ghost.erased a))
-      (c : tree_cond t pre post)
+let ghost_to_steel_steel (a : Type)
+      (t : G.erased (prog_tree (Ghost.erased a)))
+      (pre : G.erased pre_t) (post : G.erased (post_t (Ghost.erased a)))
+      (c : G.erased (tree_cond t pre post))
       ($r : repr_steel_t (SH.KGhost Set.empty) (Ghost.erased a) pre post (tree_req t c) (tree_ens t c))
   : repr_steel_t SH.KSteel (Ghost.erased a) pre post (tree_req t c) (tree_ens t c)
   = SH.steel_f (SH.ghost_u r)
-
-[@@ __repr_M__]
-inline_for_extraction noextract
-let ghost_to_steel (#a : Type) (f : repr (SH.KGhost Set.empty) (Ghost.erased a))
-  : repr SH.KSteel (Ghost.erased a)
-  = {
-    repr_tree  = f.repr_tree;
-    repr_steel = (fun pre post c ->
-                    ghost_to_steel_steel a f.repr_tree pre post c (f.repr_steel _ _ c))
-  }
-
-[@@ __repr_M__]
-inline_for_extraction noextract
-let ghost_to_steel_ct (#a : Type) (f : repr (SH.KGhost Set.empty) a)
-      (rv : (x : Ghost.erased a) -> (x' : a { x' == Ghost.reveal x }))
-  : repr SH.KSteel a
-  = repr_lift (Rt1n_trans _ _ (Lift_ghost_ghostI ({erasable_rv = rv}) _)
-              (Rt1n_trans _ _ (Lift_ghostI_atomic _)
-              (Rt1n_trans _ _ Lift_atomic_steel Rt1n_refl))) f
