experiment/Experiment.Steel.Repr.M.fst
@@ -7,11 +7,108 @@ module L = FStar.List.Pure
 
 (*** [repr_steel_t] *)
 
+// TODO? avoid the duplication due to the several Steel effects by using meta-programming
+
+inline_for_extraction noextract
+let repr_steel_subcomp__steel
+      (#a : Type) (#pre : G.erased pre_t) (#post : G.erased (post_t a))
+      (req_f : req_t pre) (ens_f : ens_t pre a post)
+      (req_g : req_t pre) (ens_g : ens_t pre a post)
+      (pf_req : (sl0 : sl_f pre) ->
+                Lemma (requires req_g sl0) (ensures req_f sl0))
+      (pf_ens : (sl0 : sl_f pre) -> (x : a) -> (sl1 : sl_f (G.reveal post x)) ->
+                Lemma (requires req_f sl0 /\ req_g sl0 /\ ens_f sl0 x sl1) (ensures ens_g sl0 x sl1))
+      (r : repr_steel_t SH.KSteel a pre post req_f ens_f)
+  : repr_steel_t SH.KSteel a pre post req_g ens_g
+  = SH.steel_f (fun () ->
+      (**) let sl0 = gget_f pre in
+      (**) pf_req sl0;
+      let x = SH.steel_u r () in
+      (**) let sl1 = gget_f (G.reveal post x) in
+      (**) pf_ens sl0 x sl1;
+      Steel.Effect.Atomic.return x)
+
+inline_for_extraction noextract
+let repr_steel_subcomp__atomic
+      (#a : Type) (opened : Mem.inames) (#pre : G.erased pre_t) (#post : G.erased (post_t a))
+      (req_f : req_t pre) (ens_f : ens_t pre a post)
+      (req_g : req_t pre) (ens_g : ens_t pre a post)
+      (pf_req : (sl0 : sl_f pre) ->
+                Lemma (requires req_g sl0) (ensures req_f sl0))
+      (pf_ens : (sl0 : sl_f pre) -> (x : a) -> (sl1 : sl_f (G.reveal post x)) ->
+                Lemma (requires req_f sl0 /\ req_g sl0 /\ ens_f sl0 x sl1) (ensures ens_g sl0 x sl1))
+      (r : repr_steel_t (SH.KAtomic opened) a pre post req_f ens_f)
+  : repr_steel_t (SH.KAtomic opened) a pre post req_g ens_g
+  = SH.atomic_f (fun () ->
+      (**) let sl0 = gget_f pre in
+      (**) pf_req sl0;
+      let x = SH.atomic_u r () in
+      (**) let sl1 = gget_f (G.reveal post x) in
+      (**) pf_ens sl0 x sl1;
+      Steel.Effect.Atomic.return x)
+
+inline_for_extraction noextract
+let repr_steel_subcomp__ghostI
+      (#a : Type) (opened : Mem.inames) (#pre : G.erased pre_t) (#post : G.erased (post_t a))
+      (req_f : req_t pre) (ens_f : ens_t pre a post)
+      (req_g : req_t pre) (ens_g : ens_t pre a post)
+      (pf_req : (sl0 : sl_f pre) ->
+                Lemma (requires req_g sl0) (ensures req_f sl0))
+      (pf_ens : (sl0 : sl_f pre) -> (x : a) -> (sl1 : sl_f (G.reveal post x)) ->
+                Lemma (requires req_f sl0 /\ req_g sl0 /\ ens_f sl0 x sl1) (ensures ens_g sl0 x sl1))
+      (r : repr_steel_t (SH.KGhostI opened) a pre post req_f ens_f)
+  : repr_steel_t (SH.KGhostI opened) a pre post req_g ens_g
+  = SH.ghostI_f (fun () ->
+      (**) let sl0 = gget_f pre in
+      (**) pf_req sl0;
+      let x = SH.ghostI_u r () in
+      (**) let sl1 = gget_f (G.reveal post x) in
+      (**) pf_ens sl0 x sl1;
+      Steel.Effect.Atomic.return x)
+
+inline_for_extraction noextract
+let repr_steel_subcomp__ghost
+      (#a : Type) (opened : Mem.inames) (#pre : G.erased pre_t) (#post : G.erased (post_t a))
+      (req_f : req_t pre) (ens_f : ens_t pre a post)
+      (req_g : req_t pre) (ens_g : ens_t pre a post)
+      (pf_req : (sl0 : sl_f pre) ->
+                Lemma (requires req_g sl0) (ensures req_f sl0))
+      (pf_ens : (sl0 : sl_f pre) -> (x : a) -> (sl1 : sl_f (G.reveal post x)) ->
+                Lemma (requires req_f sl0 /\ req_g sl0 /\ ens_f sl0 x sl1) (ensures ens_g sl0 x sl1))
+      (r : repr_steel_t (SH.KGhost opened) a pre post req_f ens_f)
+  : repr_steel_t (SH.KGhost opened) a pre post req_g ens_g
+  = SH.ghost_f (fun () ->
+      (**) let sl0 = gget_f pre in
+      (**) pf_req sl0;
+      let x = SH.ghost_u r () in
+      (**) let sl1 = gget_f (G.reveal post x) in
+      (**) pf_ens sl0 x sl1;
+      noop ();
+      x)
+
+inline_for_extraction noextract
+let repr_steel_subcomp
+      (ek : SH.effect_kind) (#a : Type) (#pre : G.erased pre_t) (#post : G.erased (post_t a))
+      (req_f : req_t pre) (ens_f : ens_t pre a post)
+      (req_g : req_t pre) (ens_g : ens_t pre a post)
+      (pf_req : (sl0 : sl_f pre) ->
+                Lemma (requires req_g sl0) (ensures req_f sl0))
+      (pf_ens : (sl0 : sl_f pre) -> (x : a) -> (sl1 : sl_f (G.reveal post x)) ->
+                Lemma (requires req_f sl0 /\ req_g sl0 /\ ens_f sl0 x sl1) (ensures ens_g sl0 x sl1))
+      (r : repr_steel_t ek a pre post req_f ens_f)
+  : repr_steel_t ek a pre post req_g ens_g
+  = match ek with
+  | SH.KSteel    -> repr_steel_subcomp__steel    req_f ens_f req_g ens_g pf_req pf_ens r
+  | SH.KAtomic o -> repr_steel_subcomp__atomic o req_f ens_f req_g ens_g pf_req pf_ens r
+  | SH.KGhostI o -> repr_steel_subcomp__ghostI o req_f ens_f req_g ens_g pf_req pf_ens r
+  | SH.KGhost  o -> repr_steel_subcomp__ghost  o req_f ens_f req_g ens_g pf_req pf_ens r
+
+
 inline_for_extraction noextract
 let steel_of_repr
       (#ek : SH.effect_kind)
       (#a : Type) (#pre : SE.pre_t) (#post : SE.post_t a) (#req : SE.req_t pre) (#ens : SE.ens_t pre a post)
-      (tr : to_repr_t a pre post req ens)
+      (tr : G.erased (to_repr_t a pre post req ens))
       (f : repr_steel_t ek a tr.r_pre tr.r_post tr.r_req tr.r_ens)
   : SH.steel a pre post req ens ek
   =
@@ -30,7 +127,7 @@ inline_for_extraction noextract
 let repr_of_steel
       (#ek : SH.effect_kind)
       (#a : Type) (#pre : SE.pre_t) (#post : SE.post_t a) (#req : SE.req_t pre) (#ens : SE.ens_t pre a post)
-      (tr : to_repr_t a pre post req ens)
+      (tr : G.erased (to_repr_t a pre post req ens))
       ($f  : SH.steel a pre post req ens ek)
   : repr_steel_t ek a tr.r_pre tr.r_post tr.r_req tr.r_ens
   =
@@ -51,8 +148,8 @@ let repr_of_steel
 #push-options "--ifuel 0 --fuel 0"
 inline_for_extraction noextract
 let spec_r_of_find_ro__steel
-      (#a : Type) (#pre : pre_t) (#post : post_t a) (#req : req_t pre) (#ens : ens_t pre a post)
-      (sro : spec_find_ro a pre post req ens)
+      (#a : Type) (#pre : G.erased pre_t) (#post : G.erased (post_t a)) (#req : req_t pre) (#ens : ens_t pre a post)
+      (sro : G.erased (spec_find_ro a pre post req ens))
       (f : repr_steel_t SH.KSteel a pre post req ens)
   : spc_steel_t SH.KSteel sro.sro_spc
   = SH.steel_f (fun () ->
@@ -62,7 +159,7 @@ let spec_r_of_find_ro__steel
       (**) change_vpl_perm sro.sro_pre_eq;
       (**) sro.sro_req_eq sl0 sl_fr0;
       let (x : a) = SH.steel_u f ()     in
-      (**) let sl1'   = gget_f (post x) in
+      (**) let sl1'   = gget_f (G.reveal post x) in
       (**) change_vpl_perm (sro.sro_post_eq x);
       (**) extract_vars_sym_l (sro.sro_post_eq x) sl1';
       (**) elim_vpl_append (sro.sro_spc.spc_post x) sro.sro_spc.spc_ro;
@@ -73,8 +170,8 @@ let spec_r_of_find_ro__steel
 
 inline_for_extraction noextract
 let spec_r_of_find_ro__atomic
-      (#a : Type) (#pre : pre_t) (#post : post_t a) (#req : req_t pre) (#ens : ens_t pre a post)
-      (sro : spec_find_ro a pre post req ens)
+      (#a : Type) (#pre : G.erased pre_t) (#post : G.erased (post_t a)) (#req : req_t pre) (#ens : ens_t pre a post)
+      (sro : G.erased (spec_find_ro a pre post req ens))
       (#opened : Mem.inames) (f : repr_steel_t (SH.KAtomic opened) a pre post req ens)
   : spc_steel_t (SH.KAtomic opened) sro.sro_spc
   = SH.atomic_f (fun () ->
@@ -84,7 +181,7 @@ let spec_r_of_find_ro__atomic
       (**) change_vpl_perm sro.sro_pre_eq;
       (**) sro.sro_req_eq sl0 sl_fr0;
       let (x : a) = SH.atomic_u f ()    in
-      (**) let sl1'   = gget_f (post x) in
+      (**) let sl1'   = gget_f (G.reveal post x) in
       (**) change_vpl_perm (sro.sro_post_eq x);
       (**) extract_vars_sym_l (sro.sro_post_eq x) sl1';
       (**) elim_vpl_append (sro.sro_spc.spc_post x) sro.sro_spc.spc_ro;
@@ -95,8 +192,8 @@ let spec_r_of_find_ro__atomic
 
 inline_for_extraction noextract
 let spec_r_of_find_ro__ghostI
-      (#a : Type) (#pre : pre_t) (#post : post_t a) (#req : req_t pre) (#ens : ens_t pre a post)
-      (sro : spec_find_ro a pre post req ens)
+      (#a : Type) (#pre : G.erased pre_t) (#post : G.erased (post_t a)) (#req : req_t pre) (#ens : ens_t pre a post)
+      (sro : G.erased (spec_find_ro a pre post req ens))
       (#opened : Mem.inames) (f : repr_steel_t (SH.KGhostI opened) a pre post req ens)
   : spc_steel_t (SH.KGhostI opened) sro.sro_spc
   = SH.ghostI_f (fun () ->
@@ -106,7 +203,7 @@ let spec_r_of_find_ro__ghostI
       (**) change_vpl_perm sro.sro_pre_eq;
       (**) sro.sro_req_eq sl0 sl_fr0;
       let (x : a) = SH.ghostI_u f ()    in
-      (**) let sl1'   = gget_f (post x) in
+      (**) let sl1'   = gget_f (G.reveal post x) in
       (**) change_vpl_perm (sro.sro_post_eq x);
       (**) extract_vars_sym_l (sro.sro_post_eq x) sl1';
       (**) elim_vpl_append (sro.sro_spc.spc_post x) sro.sro_spc.spc_ro;
@@ -117,8 +214,8 @@ let spec_r_of_find_ro__ghostI
 
 inline_for_extraction noextract
 let spec_r_of_find_ro__ghost
-      (#a : Type) (#pre : pre_t) (#post : post_t a) (#req : req_t pre) (#ens : ens_t pre a post)
-      (sro : spec_find_ro a pre post req ens)
+      (#a : Type) (#pre : G.erased pre_t) (#post : G.erased (post_t a)) (#req : req_t pre) (#ens : ens_t pre a post)
+      (sro : G.erased (spec_find_ro a pre post req ens))
       (#opened : Mem.inames) (f : repr_steel_t (SH.KGhost opened) a pre post req ens)
   : spc_steel_t (SH.KGhost opened) sro.sro_spc
   = SH.ghost_f (fun () ->
@@ -128,7 +225,7 @@ let spec_r_of_find_ro__ghost
       (**) change_vpl_perm sro.sro_pre_eq;
       (**) sro.sro_req_eq sl0 sl_fr0;
       let (x : a) = SH.ghost_u f ()    in
-      (**) let sl1'   = gget_f (post x) in
+      (**) let sl1'   = gget_f (G.reveal post x) in
       (**) change_vpl_perm (sro.sro_post_eq x);
       (**) extract_vars_sym_l (sro.sro_post_eq x) sl1';
       (**) elim_vpl_append (sro.sro_spc.spc_post x) sro.sro_spc.spc_ro;
@@ -142,8 +239,8 @@ let spec_r_of_find_ro__ghost
 
 inline_for_extraction noextract
 let spec_r_of_find_ro
-      (#a : Type) (#pre : pre_t) (#post : post_t a) (#req : req_t pre) (#ens : ens_t pre a post)
-      (sro : spec_find_ro a pre post req ens)
+      (#a : Type) (#pre : G.erased pre_t) (#post : G.erased (post_t a)) (#req : req_t pre) (#ens : ens_t pre a post)
+      (sro : G.erased (spec_find_ro a pre post req ens))
       (#ek : SH.effect_kind) (f : repr_steel_t ek a pre post req ens)
   : spc_steel_t ek sro.sro_spc
   = match ek with
