experiment/Experiment.Steel.Repr.M.fsti
@@ -1,6 +1,7 @@
 module Experiment.Steel.Repr.M
 
 module U    = Learn.Util
+module G    = FStar.Ghost
 module L    = FStar.List.Pure
 module Dl   = Learn.DList
 module Fl   = Learn.FList
@@ -36,101 +37,17 @@ type repr_steel_t (ek : SH.effect_kind) (a : Type)
       (requires fun h0 -> req (sel_f pre h0)) (ensures fun h0 x h1 -> ens (sel_f pre h0) x (sel_f (post x) h1))
       ek
 
-// FIXME: this definition fails when loaded as a dependency but not when lax-checked
 inline_for_extraction noextract
-let repr_steel_subcomp__steel
-      (#a : Type) (#pre : pre_t) (#post : post_t a)
+val repr_steel_subcomp
+      (ek : SH.effect_kind) (#a : Type) (#pre : G.erased pre_t) (#post : G.erased (post_t a))
       (req_f : req_t pre) (ens_f : ens_t pre a post)
       (req_g : req_t pre) (ens_g : ens_t pre a post)
       (pf_req : (sl0 : sl_f pre) ->
                 Lemma (requires req_g sl0) (ensures req_f sl0))
-      (pf_ens : (sl0 : sl_f pre) -> (x : a) -> (sl1 : sl_f (post x)) ->
-                Lemma (requires req_f sl0 /\ req_g sl0 /\ ens_f sl0 x sl1) (ensures ens_g sl0 x sl1))
-      (r : repr_steel_t SH.KSteel a pre post req_f ens_f)
-  : repr_steel_t SH.KSteel a pre post req_g ens_g
-  = SH.steel_f (fun () ->
-      (**) let sl0 = gget_f pre in
-      (**) pf_req (sl0);
-      let x = SH.steel_u r () in
-      (**) let sl1 = gget_f (post x) in
-      (**) pf_ens sl0 x sl1;
-      Steel.Effect.Atomic.return x)
-
-inline_for_extraction noextract
-let repr_steel_subcomp__atomic
-      (#a : Type) (opened : Mem.inames) (#pre : pre_t) (#post : post_t a)
-      (req_f : req_t pre) (ens_f : ens_t pre a post)
-      (req_g : req_t pre) (ens_g : ens_t pre a post)
-      (pf_req : (sl0 : sl_f pre) ->
-                Lemma (requires req_g sl0) (ensures req_f sl0))
-      (pf_ens : (sl0 : sl_f pre) -> (x : a) -> (sl1 : sl_f (post x)) ->
-                Lemma (requires req_f sl0 /\ req_g sl0 /\ ens_f sl0 x sl1) (ensures ens_g sl0 x sl1))
-      (r : repr_steel_t (SH.KAtomic opened) a pre post req_f ens_f)
-  : repr_steel_t (SH.KAtomic opened) a pre post req_g ens_g
-  = SH.atomic_f (fun () ->
-      (**) let sl0 = gget_f pre in
-      (**) pf_req (sl0);
-      let x = SH.atomic_u r () in
-      (**) let sl1 = gget_f (post x) in
-      (**) pf_ens sl0 x sl1;
-      Steel.Effect.Atomic.return x)
-
-inline_for_extraction noextract
-let repr_steel_subcomp__ghostI
-      (#a : Type) (opened : Mem.inames) (#pre : pre_t) (#post : post_t a)
-      (req_f : req_t pre) (ens_f : ens_t pre a post)
-      (req_g : req_t pre) (ens_g : ens_t pre a post)
-      (pf_req : (sl0 : sl_f pre) ->
-                Lemma (requires req_g sl0) (ensures req_f sl0))
-      (pf_ens : (sl0 : sl_f pre) -> (x : a) -> (sl1 : sl_f (post x)) ->
-                Lemma (requires req_f sl0 /\ req_g sl0 /\ ens_f sl0 x sl1) (ensures ens_g sl0 x sl1))
-      (r : repr_steel_t (SH.KGhostI opened) a pre post req_f ens_f)
-  : repr_steel_t (SH.KGhostI opened) a pre post req_g ens_g
-  = SH.ghostI_f (fun () ->
-      (**) let sl0 = gget_f pre in
-      (**) pf_req (sl0);
-      let x = SH.ghostI_u r () in
-      (**) let sl1 = gget_f (post x) in
-      (**) pf_ens sl0 x sl1;
-      Steel.Effect.Atomic.return x)
-
-inline_for_extraction noextract
-let repr_steel_subcomp__ghost
-      (#a : Type) (opened : Mem.inames) (#pre : pre_t) (#post : post_t a)
-      (req_f : req_t pre) (ens_f : ens_t pre a post)
-      (req_g : req_t pre) (ens_g : ens_t pre a post)
-      (pf_req : (sl0 : sl_f pre) ->
-                Lemma (requires req_g sl0) (ensures req_f sl0))
-      (pf_ens : (sl0 : sl_f pre) -> (x : a) -> (sl1 : sl_f (post x)) ->
-                Lemma (requires req_f sl0 /\ req_g sl0 /\ ens_f sl0 x sl1) (ensures ens_g sl0 x sl1))
-      (r : repr_steel_t (SH.KGhost opened) a pre post req_f ens_f)
-  : repr_steel_t (SH.KGhost opened) a pre post req_g ens_g
-  = SH.ghost_f (fun () ->
-      (**) let sl0 = gget_f pre in
-      (**) pf_req (sl0);
-      let x = SH.ghost_u r () in
-      (**) let sl1 = gget_f (post x) in
-      (**) pf_ens sl0 x sl1;
-      noop ();
-      x)
-
-inline_for_extraction noextract
-let repr_steel_subcomp
-      (ek : SH.effect_kind) (#a : Type) (#pre : pre_t) (#post : post_t a)
-      (req_f : req_t pre) (ens_f : ens_t pre a post)
-      (req_g : req_t pre) (ens_g : ens_t pre a post)
-      (pf_req : (sl0 : sl_f pre) ->
-                Lemma (requires req_g sl0) (ensures req_f sl0))
-      (pf_ens : (sl0 : sl_f pre) -> (x : a) -> (sl1 : sl_f (post x)) ->
+      (pf_ens : (sl0 : sl_f pre) -> (x : a) -> (sl1 : sl_f (G.reveal post x)) ->
                 Lemma (requires req_f sl0 /\ req_g sl0 /\ ens_f sl0 x sl1) (ensures ens_g sl0 x sl1))
       (r : repr_steel_t ek a pre post req_f ens_f)
   : repr_steel_t ek a pre post req_g ens_g
-  = match ek with
-  | SH.KSteel    -> repr_steel_subcomp__steel    req_f ens_f req_g ens_g pf_req pf_ens r
-  | SH.KAtomic o -> repr_steel_subcomp__atomic o req_f ens_f req_g ens_g pf_req pf_ens r
-  | SH.KGhostI o -> repr_steel_subcomp__ghostI o req_f ens_f req_g ens_g pf_req pf_ens r
-  | SH.KGhost  o -> repr_steel_subcomp__ghost  o req_f ens_f req_g ens_g pf_req pf_ens r
-
 
 (*// This fail, seemingly because of the expansion of the memories when checking the post
 [@@ handle_smt_goals ]
@@ -166,7 +83,7 @@ inline_for_extraction noextract
 val steel_of_repr
       (#ek : SH.effect_kind)
       (#a : Type) (#pre : SE.pre_t) (#post : SE.post_t a) (#req : SE.req_t pre) (#ens : SE.ens_t pre a post)
-      (tr : to_repr_t a pre post req ens)
+      (tr : G.erased (to_repr_t a pre post req ens))
       (f : repr_steel_t ek a tr.r_pre tr.r_post tr.r_req tr.r_ens)
   : SH.steel a pre post req ens ek
 
@@ -174,14 +91,14 @@ inline_for_extraction noextract
 val repr_of_steel
       (#ek : SH.effect_kind)
       (#a : Type) (#pre : SE.pre_t) (#post : SE.post_t a) (#req : SE.req_t pre) (#ens : SE.ens_t pre a post)
-      (tr : to_repr_t a pre post req ens)
+      (tr : G.erased (to_repr_t a pre post req ens))
       ($f  : SH.steel a pre post req ens ek)
   : repr_steel_t ek a tr.r_pre tr.r_post tr.r_req tr.r_ens 
 
 
 (*** [spec_r] *)
 
-[@@ Learn.Tactics.Util.__tac_helper__]
+[@@ Learn.Tactics.Util.__tac_helper__; Itf.__extraction__]
 noeq inline_for_extraction
 type spec_r (a : Type u#a) = {
   spc_pre  : pre_t;
@@ -243,8 +160,8 @@ let trivial_spec_find_ro a pre post req ens : spec_find_ro a pre post req ens = 
 
 inline_for_extraction noextract
 val spec_r_of_find_ro
-      (#a : Type) (#pre : pre_t) (#post : post_t a) (#req : req_t pre) (#ens : ens_t pre a post)
-      (sro : spec_find_ro a pre post req ens)
+      (#a : Type) (#pre : G.erased pre_t) (#post : G.erased (post_t a)) (#req : req_t pre) (#ens : ens_t pre a post)
+      (sro : G.erased (spec_find_ro a pre post req ens))
       (#ek : SH.effect_kind) (f : repr_steel_t ek a pre post req ens)
   : spc_steel_t ek sro.sro_spc
 
@@ -501,6 +418,7 @@ and tree_ens (#a : Type u#a) (t : prog_tree u#a u#p a)
 
 /// The [repr] type contains a representation of the program as a tree and a corresponding steel function.
 
+[@@ Itf.__extraction__]
 noeq inline_for_extraction noextract
 type repr (ek : SH.effect_kind) (a : Type) = {
   repr_tree  : prog_tree u#a u#p a;
