experiment/Experiment.Steel.Combinators.fsti
@@ -1,0 +1,434 @@
+module Experiment.Steel.Combinators
+
+module U   = Learn.Util
+module G   = FStar.Ghost
+module L   = FStar.List.Pure
+module T   = FStar.Tactics
+module SE  = Steel.Effect
+module SH  = Experiment.Steel.Steel
+module Fl  = Learn.FList
+module Mem = Steel.Memory
+module Veq = Experiment.Steel.VEquiv
+module TcS = Experiment.Steel.Tac
+
+open Steel.Effect
+open Steel.Effect.Atomic
+open Experiment.Steel.Interface
+open Experiment.Steel.VPropList
+open Experiment.Steel.Repr.M
+
+#set-options "--ifuel 1 --ide_id_info_off"
+
+/// We define a "monad" (which does not satisfy the monad laws) on [M.repr]. 
+
+unfold
+let repr_steel_tc
+      (ek : SH.effect_kind) (#a : Type) (#t : prog_tree a) (#pre : pre_t) (#post : post_t a)
+      ($tc : tree_cond t pre post)
+  : Type
+  = repr_steel_t ek a pre post (tree_req t tc) (tree_ens t tc)
+
+(****** Call *)
+
+inline_for_extraction noextract
+val tcspec_steel
+      (a : Type) (ek : SH.effect_kind)
+      (pre : G.erased pre_t) (post : G.erased (post_t a)) (ro : G.erased vprop_list)
+      (req : sl_f pre -> sl_f ro -> Type0) (ens : sl_f pre -> (x : a) -> sl_f (G.reveal post x) -> sl_f ro -> Type0)
+      (tcs : G.erased (tree_cond_Spec a L.(pre @ ro) (spc_post1 (Mkspec_r pre post ro req ens))))
+      ($f : spc_steel_t ek (Mkspec_r pre post ro req ens))
+  : repr_steel_tc ek (TCspec #a #(spec_r_exact (Mkspec_r pre post ro req ens)) _ SpecExact tcs)
+
+[@@ __repr_M__]
+let tree_of_steel_r (#ek : SH.effect_kind) (#a : Type) (#s : spec_r a) ($f : spc_steel_t ek s)
+  : prog_tree a
+  = Tspec a (spec_r_exact s)
+
+[@@ __repr_M__]
+inline_for_extraction noextract
+let repr_of_steel_r
+      (#a : Type) (s : spec_r a) (#ek : SH.effect_kind) ($f : spc_steel_t ek s)
+  : repr ek a
+  = {
+    repr_tree  = tree_of_steel_r f;
+    repr_steel = (fun pre'0 post'0 c ->
+                    let TCspec _ _ tcs = c in
+                    let Mkspec_r pre0 post0 ro0 req0 ens0 = s in
+                    tcspec_steel a ek pre0 post0 ro0 req0 ens0 tcs f)
+  }
+
+
+[@@ __repr_M__]
+let tree_of_steel
+      (#a : Type) (#pre : SE.pre_t) (#post : SE.post_t a) (#req : SE.req_t pre) (#ens : SE.ens_t pre a post)
+      (#ek : SH.effect_kind) ($f : SH.steel a pre post req ens ek)
+  : prog_tree a
+  = Tspec a (spec_r_steel pre post req ens)
+
+[@@ __repr_M__]
+inline_for_extraction noextract
+let repr_of_steel
+      (#a : Type) (pre : SE.pre_t) (post : SE.post_t a) (req : SE.req_t pre) (ens : SE.ens_t pre a post)
+      (#ek : SH.effect_kind) ($f : SH.steel a pre post req ens ek)
+  : repr ek a
+  = {
+    repr_tree  = tree_of_steel f;
+    repr_steel = (fun pre'0 post'0 c ->
+                    let TCspec #a #sp s sh tcs = c in
+                    let SpecSteel tr (Mkspec_find_ro (Mkspec_r pre0 post0 ro0 req0 ens0)
+                                                     pre_eq post_eq req_eq ens_eq)
+                      = U.cast (spec_r_steel pre post req ens s) sh in
+                    let sr = Mkspec_find_ro (Mkspec_r pre0 post0 ro0 req0 ens0)
+                                            pre_eq post_eq req_eq ens_eq in
+                    tcspec_steel a ek pre0 post0 ro0 req0 ens0 tcs
+                       (spec_r_of_find_ro #a #tr.r_pre #tr.r_post #tr.r_req #tr.r_ens sr (repr_of_steel tr f)))
+  }
+
+
+(****** Return *)
+
+inline_for_extraction noextract
+val return_steel
+      (a : Type) (ek : SH.effect_kind) (x : a) (sl_hint : option (post_t a))
+      (pre : G.erased pre_t) (post : G.erased (post_t a))
+      (e : Veq.vequiv pre (G.reveal post x))
+  : repr_steel_tc ek (TCret #a #x #sl_hint pre post e)
+
+[@@ __repr_M__]
+inline_for_extraction noextract
+let return_hint (ek : SH.effect_kind) (#a : Type) (x : a) (sl_hint : option (post_t a))
+  : repr ek a
+  = {
+    repr_tree  = Tret a x sl_hint;
+    repr_steel = (fun pre0 post0 c ->
+        let TCret pre post p = c in
+        return_steel a ek x sl_hint pre post p)
+  }
+
+[@@ __repr_M__]
+inline_for_extraction noextract
+let return (ek : SH.effect_kind) (#a : Type) (x : a) : repr ek a
+  = return_hint ek x None
+
+
+(****** Bind *)
+
+type bind_steel_t (ek0 ek1 ek2 : SH.effect_kind) =
+      (a : Type) ->  (b : Type) -> (f : G.erased (prog_tree a)) -> (g : G.erased (a -> prog_tree b)) ->
+      (pre : G.erased pre_t) -> (itm : G.erased (post_t a)) -> (post : G.erased (post_t b)) ->
+      (cf : G.erased (tree_cond f pre itm)) ->
+      (cg : G.erased ((x : a) -> tree_cond (G.reveal g x) (G.reveal itm x) post)) ->
+      (rf : repr_steel_tc ek0 cf) ->
+      (rg : ((x : a) -> repr_steel_tc ek1 (G.reveal cg x))) ->
+      repr_steel_tc ek2 (TCbind #a #b #f #g pre itm post cf cg)
+
+inline_for_extraction noextract
+val bind_steel__steel
+  : bind_steel_t SH.KSteel SH.KSteel SH.KSteel
+
+inline_for_extraction noextract
+val bind_steel__atomic_ghost (o : Mem.inames)
+  : bind_steel_t (SH.KAtomic o) (SH.KGhostI o) (SH.KAtomic o)
+
+inline_for_extraction noextract
+val bind_steel__ghost_atomic (o : Mem.inames)
+  : bind_steel_t (SH.KGhostI o) (SH.KAtomic o) (SH.KAtomic o)
+
+inline_for_extraction noextract
+val bind_steel__ghostI (o : Mem.inames)
+  : bind_steel_t (SH.KGhostI o) (SH.KGhostI o) (SH.KGhostI o)
+
+inline_for_extraction noextract
+val bind_steel__ghost(o : Mem.inames)
+  : bind_steel_t (SH.KGhost o) (SH.KGhost o) (SH.KGhost o)
+
+(**) private val end_bind_steel : unit
+
+[@@ __repr_M__]
+inline_for_extraction noextract
+let bind_ek (#a #b : Type) (ek0 ek1 ek2 : SH.effect_kind) (s : bind_steel_t ek0 ek1 ek2)
+      (f : repr ek0 a) (g : a -> repr ek1 b)
+  : repr ek2 b
+  = {
+    repr_tree  = Tbind a b f.repr_tree (fun x -> (g x).repr_tree);
+    repr_steel = (fun pre0 post0 c ->
+                    let (TCbind #a' #b' #tf #tg pre itm post cf cg) = c in
+                    let rg (x : a) : repr_steel_t ek1 b (itm x) post _ _
+                                   = (g x).repr_steel _ _ (cg x) in
+                    s a b tf tg pre itm post cf cg (f.repr_steel _ _ cf) rg)
+  }
+
+[@@ __repr_M__]
+inline_for_extraction noextract
+let bind (#a #b : Type) (f : repr SH.KSteel a) (g : a -> repr SH.KSteel b)
+  : repr SH.KSteel b
+  = bind_ek SH.KSteel SH.KSteel SH.KSteel bind_steel__steel f g
+
+[@@ __repr_M__]
+inline_for_extraction noextract
+let bind_ghost (#a #b : Type) (#opened : Mem.inames)
+               (f : repr (SH.KGhost opened) a) (g : a -> repr (SH.KGhost opened) b)
+  : repr (SH.KGhost opened) b
+  = bind_ek (SH.KGhost opened) (SH.KGhost opened) (SH.KGhost opened) (bind_steel__ghost opened) f g
+
+
+(****** Bind pure *)
+
+inline_for_extraction noextract
+val bindP_steel__ghost
+      (a : Type) (b : Type) (opened : Mem.inames) (wp : pure_wp a) ($f : unit -> GHOST a wp)
+      (g : G.erased (a -> prog_tree b))
+      (pre : G.erased pre_t) (post : G.erased (post_t b))
+      (cg : G.erased ((x : a) -> tree_cond (G.reveal g x) pre post))
+      (rg : (x : a) -> repr_steel_tc (SH.KGhost opened) (G.reveal cg x))
+  : repr_steel_tc (SH.KGhost opened) (TCbindP #a #b #wp #g pre post cg)
+
+inline_for_extraction noextract
+val bindP_steel
+      (a : Type) (b : Type) (ek : SH.effect_kind) (wp : pure_wp a) ($f : unit -> PURE a wp)
+      (g : G.erased (a -> prog_tree b))
+      (pre : G.erased pre_t) (post : G.erased (post_t b))
+      (cg : ((x : a) -> tree_cond (G.reveal g x) pre post))
+      (rg : (x : a) -> repr_steel_tc ek (G.reveal cg x))
+  : repr_steel_tc ek (TCbindP #a #b #wp #g pre post cg)
+
+#push-options "--ifuel 1 --fuel 1 --z3rlimit 10"
+[@@ __repr_M__]
+inline_for_extraction noextract
+let bindP (#a #b : Type) (ek : SH.effect_kind) (wp : pure_wp a) ($f : unit -> PURE a wp) (g : a -> repr ek b)
+  : repr ek b
+  = {
+    repr_tree  = TbindP a b wp (fun x -> (g x).repr_tree);
+    repr_steel = (fun pre0 post0 c ->
+                    let (TCbindP #a' #b' #wp #tg pre post cg) = c in
+                    let rg (x : a) : repr_steel_t ek b pre post _ _
+                                   = (g x).repr_steel _ _ (cg x) in
+                    bindP_steel a b ek wp f tg pre post cg rg)
+  }
+
+[@@ __repr_M__]
+inline_for_extraction noextract
+let bindP_ghost (#a #b : Type) (#opened : Mem.inames)
+                (wp : pure_wp a) ($f : unit -> GHOST a wp) (g : a -> repr (SH.KGhost opened) b)
+  : repr (SH.KGhost opened) b
+  = {
+    repr_tree  = TbindP a b wp (fun x -> (g x).repr_tree);
+    repr_steel = (fun pre0 post0 c ->
+                    let (TCbindP #a' #b' #wp #tg pre post cg) = c in
+                    let rg (x : a) : repr_steel_t (SH.KGhost opened) b pre post _ _
+                                   = (g x).repr_steel _ _ (cg x) in
+                    bindP_steel__ghost a b opened wp f tg pre post cg rg)
+  }
+#pop-options
+
+
+(****** If-then-else *)
+
+inline_for_extraction noextract
+val ite_steel
+      (a : Type) (guard : bool)
+      (thn  : G.erased (prog_tree a)) (els : G.erased (prog_tree a))
+      (pre  : G.erased pre_t) (post : G.erased (post_t a))
+      (cthn : G.erased (tree_cond thn pre post))
+      (cels : G.erased (tree_cond els pre post))
+      (rthn : repr_steel_tc SH.KSteel cthn)
+      (rels : repr_steel_tc SH.KSteel cels)
+  : repr_steel_tc SH.KSteel (TCif #a #guard #thn #els pre post cthn cels)
+
+inline_for_extraction noextract
+val ite_ghost_steel
+      (a : Type) (opened : Mem.inames) (guard : bool)
+      (thn  : G.erased (prog_tree a)) (els : G.erased (prog_tree a))
+      (pre  : G.erased pre_t) (post : G.erased (post_t a))
+      (cthn : G.erased (tree_cond thn pre post))
+      (cels : G.erased (tree_cond els pre post))
+      (rthn : repr_steel_tc (SH.KGhost opened) cthn)
+      (rels : repr_steel_tc (SH.KGhost opened) cels)
+  : repr_steel_tc (SH.KGhost opened) (TCif #a #guard #thn #els pre post cthn cels)
+
+
+[@@ __repr_M__]
+inline_for_extraction noextract
+let ite (#a : Type) (guard : bool) (thn els : repr SH.KSteel a)
+  : repr SH.KSteel a
+  = {
+    repr_tree  = Tif a guard thn.repr_tree els.repr_tree;
+    repr_steel = (fun pre0 post0 c ->
+                    let TCif pre post cthn cels = c in
+                    ite_steel a guard _ _ pre post cthn cels
+                       (thn.repr_steel _ _ cthn) (els.repr_steel _ _ cels))
+  }
+
+[@@ __repr_M__]
+inline_for_extraction noextract
+let ite_ghost (#a : Type) (#opened : Mem.inames) (guard : bool) (thn els : repr (SH.KGhost opened) a)
+  : repr (SH.KGhost opened) a
+  = {
+    repr_tree  = Tif a guard thn.repr_tree els.repr_tree;
+    repr_steel = (fun pre0 post0 c ->
+                    let (TCif pre post cthn cels) = c in
+                    ite_ghost_steel a opened guard _ _ pre post cthn cels
+                       (thn.repr_steel _ _ cthn) (els.repr_steel _ _ cels))
+  }
+
+
+
+(*** Lifts *)
+
+(***** [erasable_t] *)
+
+type revealed_value (#a : Type) (x : Ghost.erased a) =
+  x' : a { x' == Ghost.reveal x }
+
+[@@ __extraction__]
+noeq inline_for_extraction noextract
+type erasable_t (a : Type) = {
+  erasable_rv : (x : Ghost.erased a) -> revealed_value x
+}
+
+private
+let __build_revealed_value (a : Type) : (x : Ghost.erased a) -> GTot (revealed_value x)
+  = fun x -> Ghost.reveal x
+
+/// Solves a goal [erasable_t a] if a is an erasable type.
+let build_erasable_t fr ctx : T.Tac unit
+  = T.(
+    let a : term
+      = match inspect (cur_goal ()) with
+        | Tv_App  _ arg -> arg._1
+        | _ -> fail "build_erasable_t : goal"
+    in
+    apply (`Mkerasable_t);
+    // The following requires a conversion from [_ -> GTot (revealed_value x)] to [_ -> Tot (revealed_value x)]
+    // which succeeds iff [revealed_value x] (i.e. [a]) is erasable.
+    // Since we use (`#a), this may generate some guards to retypecheck (`#a).
+    with_policy SMT (fun () -> TcS.cs_try (fun () ->
+      exact (`(__build_revealed_value (`#a) <: _ -> Tot _)))
+    fr ctx (fun m -> fail (m (Fail_not_erasable a) [])))
+  )
+
+private
+let test_erasable_unit : erasable_t unit
+  = _ by (build_erasable_t default_flags TcS.dummy_ctx)
+
+private
+let test_erasable_unit' : erasable_t U.unit'
+  = _ by (build_erasable_t default_flags TcS.dummy_ctx)
+
+#push-options "--silent"
+[@@ expect_failure [228]]
+private
+let test_erasable_int : erasable_t int
+  = _ by (build_erasable_t default_flags TcS.dummy_ctx)
+#pop-options
+
+[@@ erasable]
+private noeq
+type test_guard_type (_ : squash (forall (n : nat) . n >= 0)) =
+
+private
+let test_erasable_guard : erasable_t (test_guard_type ())
+  = _ by (build_erasable_t default_flags TcS.dummy_ctx)
+
+
+(***** [steel_liftable] *)
+
+// named as in Coq
+noeq
+type clos_refl_trans_1n (#a : Type) (r : a -> a -> Type) (x : a) : a -> Type =
+  | Rt1n_refl  : clos_refl_trans_1n r x x
+  | Rt1n_trans : (y : a) -> (z : a) ->
+                 r x y -> clos_refl_trans_1n r y z -> clos_refl_trans_1n r x z
+
+noeq
+type steel_liftable1 (a : Type) : SH.effect_kind -> SH.effect_kind -> Type =
+  | Lift_ghost_ghostI  : erasable_t a -> (opened : Mem.inames) ->
+                         steel_liftable1 a (SH.KGhost     opened) (SH.KGhostI opened)
+  | Lift_ghostI_atomic : (opened : Mem.inames) ->
+                         steel_liftable1 a (SH.KGhostI    opened) (SH.KAtomic opened)
+  | Lift_atomic_steel  : steel_liftable1 a (SH.KAtomic Set.empty)  SH.KSteel
+
+type steel_liftable (a : Type) : SH.effect_kind -> SH.effect_kind -> Type
+  = clos_refl_trans_1n (steel_liftable1 a)
+
+
+/// We define the lift on [repr_steel_t] rather than on [SH.steel] because the latter option does not work
+/// with steel's tactic because of the abstract specifications.
+
+let repr_steel_lift_t (a : Type) (ek0 ek1 : SH.effect_kind) =
+  (pre : G.erased pre_t) -> (post : G.erased (post_t a)) ->
+  (req : req_t pre) -> (ens : ens_t pre a post) ->
+  (f : repr_steel_t ek0 a pre post req ens) ->
+  repr_steel_t ek1 a pre post req ens
+    
+inline_for_extraction noextract
+val repr_steel_lift_ghost_ghostI (a : Type) (opened : Mem.inames) (e : erasable_t a)
+  : repr_steel_lift_t a (SH.KGhost opened) (SH.KGhostI opened)
+
+inline_for_extraction noextract
+val repr_steel_lift_ghostI_atomic (a : Type) (opened : Mem.inames)
+  : repr_steel_lift_t a (SH.KGhostI opened) (SH.KAtomic opened)
+
+inline_for_extraction noextract
+val repr_steel_lift_atomic_steel (a : Type)
+  : repr_steel_lift_t a (SH.KAtomic Set.empty) SH.KSteel
+
+[@@ __extraction__]
+inline_for_extraction noextract
+let repr_steel_lift1
+      (#a : Type) (#pre : pre_t) (#post : post_t a) (#req : req_t pre) (#ens : ens_t pre a post)
+      (#ek0 #ek1 : SH.effect_kind) (l : steel_liftable1 a ek0 ek1)
+      (f : repr_steel_t ek0 a pre post req ens)
+  : repr_steel_t ek1 a pre post req ens
+  = match l with
+  | Lift_ghost_ghostI e o -> repr_steel_lift_ghost_ghostI  a o e pre post req ens f
+  | Lift_ghostI_atomic  o -> repr_steel_lift_ghostI_atomic a o   pre post req ens f
+  | Lift_atomic_steel     -> repr_steel_lift_atomic_steel  a     pre post req ens f
+
+[@@ __extraction__]
+inline_for_extraction noextract
+let rec repr_steel_lift
+      (#a : Type) (#pre : pre_t) (#post : post_t a) (#req : req_t pre) (#ens : ens_t pre a post)
+      (#ek0 #ek1 : SH.effect_kind) (l : steel_liftable a ek0 ek1)
+      (f : repr_steel_t ek0 a pre post req ens)
+  : Tot (repr_steel_t ek1 a pre post req ens) (decreases l)
+  = match l with
+  | Rt1n_refl -> f
+  | Rt1n_trans _ _ l0 l1 -> repr_steel_lift l1 (repr_steel_lift1 l0 f)
+
+[@@ __repr_M__]
+inline_for_extraction noextract
+let repr_lift
+      (#a : Type) (#ek0 #ek1 : SH.effect_kind) (l : steel_liftable a ek0 ek1) (r : repr ek0 a)
+  : repr ek1 a
+  = { r with repr_steel = (fun pre post c -> repr_steel_lift l (r.repr_steel pre post c)) }
+
+
+(****** SteelGhost to Steel (Monad) *)
+
+inline_for_extraction noextract
+val ghost_to_steel_steel (a : Type)
+      (t : G.erased (prog_tree (Ghost.erased a)))
+      (pre : G.erased pre_t) (post : G.erased (post_t (Ghost.erased a)))
+      (c : G.erased (tree_cond t pre post))
+      ($r : repr_steel_tc (SH.KGhost Set.empty) c)
+  : repr_steel_t SH.KSteel (Ghost.erased a) pre post (tree_req t c) (tree_ens t c)
+
+[@@ __repr_M__]
+inline_for_extraction noextract
+let ghost_to_steel (#a : Type) (f : repr (SH.KGhost Set.empty) (Ghost.erased a))
+  : repr SH.KSteel (Ghost.erased a)
+  = {
+    repr_tree  = f.repr_tree;
+    repr_steel = (fun pre post c ->
+                    ghost_to_steel_steel a f.repr_tree pre post c (f.repr_steel _ _ c))
+  }
+
+[@@ __repr_M__]
+inline_for_extraction noextract
+let ghost_to_steel_ct (#a : Type) (f : repr (SH.KGhost Set.empty) a)
+      (rv : (x : Ghost.erased a) -> (x' : a { x' == Ghost.reveal x }))
+  : repr SH.KSteel a
+  = repr_lift (Rt1n_trans _ _ (Lift_ghost_ghostI ({erasable_rv = rv}) _)
+              (Rt1n_trans _ _ (Lift_ghostI_atomic _)
+              (Rt1n_trans _ _ Lift_atomic_steel Rt1n_refl))) f
