experiment/Experiment.Steel.GCombinators.Lib.fst
@@ -1,77 +1,44 @@
 module Experiment.Steel.GCombinators.Lib
 
-include Experiment.Steel.Tac
-include Experiment.Steel.Tac.LV
-
-module U      = Learn.Util
-module L      = FStar.List.Pure
-module M      = Experiment.Steel.Repr.M
-module Ll     = Learn.List
-module Fl     = Learn.FList
-module SH     = Experiment.Steel.Steel
-module LV     = Experiment.Steel.Repr.LV
-module SF     = Experiment.Steel.Repr.SF
-module SA     = Steel.Effect.Atomic
-module Veq    = Experiment.Steel.VEquiv
-module Fun    = Experiment.Repr.Fun
-module Mem    = Steel.Memory
-module Msk    = Learn.List.Mask
-module Perm   = Learn.Permutation
-module LV2M   = Experiment.Steel.Repr.LV_to_M
-module LV2SF  = Experiment.Steel.Repr.LV_to_SF
-module SF2Fun = Experiment.Steel.Repr.SF_to_Fun
-
-open Steel.Effect
-open Steel.Effect.Atomic
-open Experiment.Steel.VPropList
-open Experiment.Steel.Interface
-open FStar.Tactics
+module L = FStar.List.Pure
+module M = Experiment.Steel.Repr.M
 
 #set-options "--fuel 1 --ifuel 1"
 
+(**** [make_combinator_steel] *)
 
-let __delta_perm : list string = [
-    `%Perm.perm_f_to_list; `%Perm.comp; `%Perm.perm_f_append; `%Perm.mk_perm_f; `%Perm.perm_f_of_pair;
-    `%Perm.pequiv_append_swap; `%Perm.pequiv_refl; `%Perm.id_n;
-    `%LV.eij_equiv; `%LV.eij_equiv_f
-  ]
-
-(*** [make_combinator] *)
-
-/// [make_combinator] is used to build a new combinator. It handle the [pre_eq] and [post_eq] of [M.TCgen].
-
-#push-options "--fuel 0 --ifuel 0"
+#push-options "--fuel 0 --ifuel 0 --z3rlimit 30"
 inline_for_extraction
-let make_combinator_steel
-      (#a : Type u#a) (s : M.spec_r a) (f : M.spc_steel_t SH.KSteel s)
-      (#pre : M.pre_t) (pre_eq : Veq.vequiv pre (M.spc_pre1 s))
-      (#post : M.post_t a) (post_eq : ((x : a) -> Veq.vequiv (M.spc_post1 s x) (post x)))
+let make_combinator_steel__steel
+      (#a : Type u#a) (s : G.erased (M.spec_r a)) (f : M.spc_steel_t SH.KSteel s)
+      (#pre : G.erased M.pre_t) (pre_eq : Veq.vequiv pre (M.spc_pre1 s))
+      (#post : G.erased (M.post_t a)) (post_eq : ((x : a) -> Veq.vequiv (M.spc_post1 s x) (G.reveal post x)))
   : M.repr_steel_t SH.KSteel a pre post (M.gen_req s pre_eq post_eq) (M.gen_ens s pre_eq post_eq)
   =
-    SH.steel_f (fun () ->
+    SH.steel_f M.(fun () ->
       pre_eq.veq_g _;
       (**) elim_vpl_append s.spc_pre s.spc_ro;
       (**) let sl0'  = gget_f s.spc_pre in
       (**) let sl_ro = gget_f s.spc_ro in     
-      (**) assert (s.spc_req sl0' sl_ro);
+      (**) assert (s.M.spc_req sl0' sl_ro);
       let (x : a) = SH.steel_u f () in
       (**) let sl1'   = gget_f (s.spc_post x) in
       (**) let sl_ro' = gget_f s.spc_ro       in
       (**) assert (sl_ro' == sl_ro);
-      (**) assert (s.spc_ens sl0' x sl1' sl_ro);
+      (**) assert (s.M.spc_ens sl0' x sl1' sl_ro);
       (**) intro_vpl_append (s.spc_post x) s.spc_ro;
       (post_eq x).veq_g _;
       SA.return x
     )
 
 inline_for_extraction
-let make_combinator_steel_atomic
-      (#a : Type u#a) (opened : Mem.inames) (s : M.spec_r a) (f : M.spc_steel_t (SH.KAtomic opened) s)
-      (#pre : M.pre_t) (pre_eq : Veq.vequiv pre (M.spc_pre1 s))
-      (#post : M.post_t a) (post_eq : ((x : a) -> Veq.vequiv (M.spc_post1 s x) (post x)))
+let make_combinator_steel__atomic
+      (#a : Type u#a) (opened : Mem.inames) (s : G.erased (M.spec_r a)) (f : M.spc_steel_t (SH.KAtomic opened) s)
+      (#pre : G.erased M.pre_t) (pre_eq : Veq.vequiv pre (M.spc_pre1 s))
+      (#post : G.erased (M.post_t a)) (post_eq : ((x : a) -> Veq.vequiv (M.spc_post1 s x) (G.reveal post x)))
   : M.repr_steel_t (SH.KAtomic opened) a pre post (M.gen_req s pre_eq post_eq) (M.gen_ens s pre_eq post_eq)
   =
-    SH.atomic_f #opened (fun () ->
+    SH.atomic_f #opened M.(fun () ->
       pre_eq.veq_g _;
       (**) elim_vpl_append s.spc_pre s.spc_ro;
       (**) let sl0'  = gget_f s.spc_pre in
@@ -88,36 +55,13 @@ let make_combinator_steel_atomic
     )
 
 inline_for_extraction
-let make_combinator_steel_ghost
-      (#a : Type u#a) (opened : Mem.inames) (s : M.spec_r a) (f : M.spc_steel_t (SH.KGhost opened) s)
-      (#pre : M.pre_t) (pre_eq : Veq.vequiv pre (M.spc_pre1 s))
-      (#post : M.post_t a) (post_eq : ((x : a) -> Veq.vequiv (M.spc_post1 s x) (post x)))
-  : M.repr_steel_t (SH.KGhost opened) a pre post (M.gen_req s pre_eq post_eq) (M.gen_ens s pre_eq post_eq)
-  =
-    SH.ghost_f #opened (fun () ->
-      pre_eq.veq_g _;
-      (**) elim_vpl_append s.spc_pre s.spc_ro;
-      (**) let sl0'  = gget_f s.spc_pre in
-      (**) let sl_ro = gget_f s.spc_ro in     
-      (**) assert (s.spc_req sl0' sl_ro);
-      let (x : a) = SH.ghost_u f () in
-      (**) let sl1'   = gget_f (s.spc_post x) in
-      (**) let sl_ro' = gget_f s.spc_ro       in
-      (**) assert (sl_ro' == sl_ro);
-      (**) assert (s.spc_ens sl0' x sl1' sl_ro);
-      (**) intro_vpl_append (s.spc_post x) s.spc_ro;
-      (post_eq x).veq_g _;
-      x
-    )
-
-inline_for_extraction
-let make_combinator_steel_ghostI
-      (#a : Type u#a) (opened : Mem.inames) (s : M.spec_r a) (f : M.spc_steel_t (SH.KGhostI opened) s)
-      (#pre : M.pre_t) (pre_eq : Veq.vequiv pre (M.spc_pre1 s))
-      (#post : M.post_t a) (post_eq : ((x : a) -> Veq.vequiv (M.spc_post1 s x) (post x)))
+let make_combinator_steel__ghostI
+      (#a : Type u#a) (opened : Mem.inames) (s : G.erased (M.spec_r a)) (f : M.spc_steel_t (SH.KGhostI opened) s)
+      (#pre : G.erased M.pre_t) (pre_eq : Veq.vequiv pre (M.spc_pre1 s))
+      (#post : G.erased (M.post_t a)) (post_eq : ((x : a) -> Veq.vequiv (M.spc_post1 s x) (G.reveal post x)))
   : M.repr_steel_t (SH.KGhostI opened) a pre post (M.gen_req s pre_eq post_eq) (M.gen_ens s pre_eq post_eq)
   =
-    SH.ghostI_f #opened (fun () ->
+    SH.ghostI_f #opened M.(fun () ->
       pre_eq.veq_g _;
       (**) elim_vpl_append s.spc_pre s.spc_ro;
       (**) let sl0'  = gget_f s.spc_pre in
@@ -132,184 +76,71 @@ let make_combinator_steel_ghostI
       (post_eq x).veq_g _;
       SA.return x
     )
+
+inline_for_extraction
+let make_combinator_steel__ghost
+      (#a : Type u#a) (opened : Mem.inames) (s : G.erased (M.spec_r a)) (f : M.spc_steel_t (SH.KGhost opened) s)
+      (#pre : G.erased M.pre_t) (pre_eq : Veq.vequiv pre (M.spc_pre1 s))
+      (#post : G.erased (M.post_t a)) (post_eq : ((x : a) -> Veq.vequiv (M.spc_post1 s x) (G.reveal post x)))
+  : M.repr_steel_t (SH.KGhost opened) a pre post (M.gen_req s pre_eq post_eq) (M.gen_ens s pre_eq post_eq)
+  =
+    SH.ghost_f #opened M.(fun () ->
+      pre_eq.veq_g _;
+      (**) elim_vpl_append s.spc_pre s.spc_ro;
+      (**) let sl0'  = gget_f s.spc_pre in
+      (**) let sl_ro = gget_f s.spc_ro in     
+      (**) assert (s.spc_req sl0' sl_ro);
+      let (x : a) = SH.ghost_u f () in
+      (**) let sl1'   = gget_f (s.spc_post x) in
+      (**) let sl_ro' = gget_f s.spc_ro       in
+      (**) assert (sl_ro' == sl_ro);
+      (**) assert (s.spc_ens sl0' x sl1' sl_ro);
+      (**) intro_vpl_append (s.spc_post x) s.spc_ro;
+      (post_eq x).veq_g _;
+      x
+    )
 #pop-options
 
 inline_for_extraction
-let make_combinator_steel_ek
-      (ek : SH.effect_kind) (#a : Type u#a) (s : M.spec_r a) (f : M.spc_steel_t ek s)
-      (#pre : M.pre_t) (pre_eq : Veq.vequiv pre (M.spc_pre1 s))
-      (#post : M.post_t a) (post_eq : ((x : a) -> Veq.vequiv (M.spc_post1 s x) (post x)))
+let make_combinator_steel
+      (ek : SH.effect_kind) (#a : Type u#a) (s : G.erased (M.spec_r a)) (f : M.spc_steel_t ek s)
+      (#pre : G.erased M.pre_t) (pre_eq : Veq.vequiv pre (M.spc_pre1 s))
+      (#post : G.erased (M.post_t a)) (post_eq : ((x : a) -> Veq.vequiv (M.spc_post1 s x) (G.reveal post x)))
   : M.repr_steel_t ek a pre post (M.gen_req s pre_eq post_eq) (M.gen_ens s pre_eq post_eq)
   = match ek with
-  | SH.KSteel         -> make_combinator_steel               s f pre_eq post_eq
-  | SH.KAtomic opened -> make_combinator_steel_atomic opened s f pre_eq post_eq
-  | SH.KGhost  opened -> make_combinator_steel_ghost  opened s f pre_eq post_eq
-  | SH.KGhostI opened -> make_combinator_steel_ghostI opened s f pre_eq post_eq
-
-[@@ __repr_M__]
-inline_for_extraction
-let make_combinator
-      (a : Type) (ek : SH.effect_kind) (gen_tac : M.gen_tac_t) (gen_c : M.spec_r a -> Type u#(max a p 2))
-      (f : (s : M.spec_r a) -> (sh : gen_c s) -> M.spc_steel_t ek s)
-  : M.repr u#a u#p ek a
-  = {
-    repr_tree  = M.Tgen a gen_tac gen_c;
-    repr_steel = (fun pre post c ->
-                    let M.TCgen s sh _ pre_eq _ post_eq = c in
-                    make_combinator_steel_ek ek s (f s sh) pre_eq post_eq)
-  }
-
-
-(*** [gen_sf_Tspec] *)
-
-/// A [LV.gen_sf] can always be built using a [SF.Tspec] with the expected specifications.
-
-#push-options "--fuel 1"
-[@@ __LV2SF__]
-let gen_sf_Tspec (#a : Type) (s : M.spec_r a)
-  : LV.gen_sf s
-  = fun (sl0 : sl_f s.spc_pre) (sl_ro : sl_f s.spc_ro) ->
-    SF.Tspec a (M.post_sl_t s.spc_post)
-             (requires s.spc_req sl0 sl_ro)
-             (ensures  fun x sl1 -> s.spc_ens sl0 x sl1 sl_ro)
-#pop-options
-
-
-(*** [lc_spec_r] *)
-
-/// [lc_spec_r lc] is the specification (given as a [M.spec_r]) resulting from the [LV.lin_cond] [lc].
-/// [lc_sf] provides a corresponding [gen_sf] (that is a [SF.prog_tree] with an equivalent specification).
-/// [lc_wp] provides a sound (but theoretically not complete) weakest-precondition.
-/// [lc_to_spc_steel_t] gives a Steel implementation.
-
-[@@ __cond_solver__; __LV2SF__]
-let lc_pre
-      (#a : Type) (#env : vprop_list) (#t : M.prog_tree a) (#csm : LV.csm_t env) (#prd : LV.prd_t a)
-      (lc : LV.lin_cond u#a u#p env t csm prd)
-  : M.pre_t
-  = Msk.(filter_mask csm env)
-
-[@@ __cond_solver__; __LV2SF__]
-let lc_post
-      (#a : Type) (#env : vprop_list) (#t : M.prog_tree a) (#csm : LV.csm_t env) (#prd : LV.prd_t a)
-      (lc : LV.lin_cond u#a u#p env t csm prd)
-  : M.post_t a
-  = prd
-
-[@@ __cond_solver__; __LV2SF__]
-let lc_ro
-      (#a : Type) (#env : vprop_list) (#t : M.prog_tree a) (#csm : LV.csm_t env) (#prd : LV.prd_t a)
-      (lc : LV.lin_cond u#a u#p env t csm prd)
-  : vprop_list
-  = Msk.(filter_mask (mask_not csm) env)
-
-let lc_req
-      (#a : Type) (#env : vprop_list) (#t : M.prog_tree a) (#csm : LV.csm_t env) (#prd : LV.prd_t a)
-      (lc : LV.lin_cond u#a u#p env t csm prd)
-      (sl0 : sl_f (lc_pre lc)) (sl_ro : sl_f (lc_ro lc))
-  : Type0
-  = LV.tree_req lc (append_vars_mask csm sl0 sl_ro)
-
-let lc_ens
-      (#a : Type) (#env : vprop_list) (#t : M.prog_tree a) (#csm : LV.csm_t env) (#prd : LV.prd_t a)
-      (lc : LV.lin_cond u#a u#p env t csm prd)
-      (sl0 : sl_f (lc_pre lc)) (x : a) (sl1 : sl_f (lc_post lc x)) (sl_ro : sl_f (lc_ro lc))
-  : Type0
-  = LV.tree_ens lc (append_vars_mask csm sl0 sl_ro) x sl1
-
-let lc_spec_r
-      (#a : Type) (#env : vprop_list) (#t : M.prog_tree a) (#csm : LV.csm_t env) (#prd : LV.prd_t a)
-      (lc : LV.lin_cond u#a u#p env t csm prd)
-  : M.spec_r a
-  = M.Mkspec_r (lc_pre lc) (lc_post lc) (lc_ro lc) (lc_req lc) (lc_ens lc)
-
-
-(***** [lc_sf] *)
-
-[@@ __LV2SF__]
-let lc_sf
-      (#a : Type) (#env : vprop_list) (#t : M.prog_tree a) (#csm : LV.csm_t env) (#prd : LV.prd_t a)
-      (lc : LV.lin_cond u#a u#p env t csm prd)
-  : LV.gen_sf (lc_spec_r lc)
-  =
-    fun (sl0 : sl_f (lc_pre lc)) (sl_ro : sl_f (lc_ro lc)) ->
-      let sl0' = LV2SF.append_vars_mask_l csm (Fl.dlist_of_f sl0) (Fl.dlist_of_f sl_ro) in
-      (**) LV2SF.repr_SF_of_LV_sound lc sl0';
-      LV2SF.repr_SF_of_LV lc sl0'
-
-let rew_lc_sf_req
-      (#a : Type) (#env : vprop_list) (#t : M.prog_tree a) (#csm : LV.csm_t env) (#prd : LV.prd_t a)
-      (lc : LV.lin_cond u#a u#p env t csm prd)
-      (sl0 : sl_f (lc_pre lc)) (sl_ro : sl_f (lc_ro lc))
-  : squash (lc_req lc sl0 sl_ro <==> SF.tree_req (lc_sf lc sl0 sl_ro))
-  = ()
-
-let rew_lc_sf_ens
-      (#a : Type) (#env : vprop_list) (#t : M.prog_tree a) (#csm : LV.csm_t env) (#prd : LV.prd_t a)
-      (lc : LV.lin_cond u#a u#p env t csm prd)
-      (sl0 : sl_f (lc_pre lc)) (x : a) (sl1 : sl_f (lc_post lc x)) (sl_ro : sl_f (lc_ro lc))
-  : squash (lc_ens lc sl0 x sl1 sl_ro <==> SF.tree_ens (lc_sf lc sl0 sl_ro) x sl1)
-  = ()
-
-
-(***** [lc_wp] *)
-
-// We mark [lc_wp] as GTot to avoid a "Substitution must be fully applied" error from F* when
-// extracting the .krml of a module that depends on this one.
-[@@ __LV2SF__]
-let lc_wp
-      (#a : Type) (#env : vprop_list) (#t : M.prog_tree a) (#csm : LV.csm_t env) (#prd : LV.prd_t a)
-      (lc : LV.lin_cond u#a u#p env t csm prd)
-      (sl0 : sl_f (lc_pre lc)) (sl_ro : sl_f (lc_ro lc))
-  : GTot (pure_wp SF2Fun.(sl_tys_v ({val_t = a; sel_t = M.post_sl_t prd})))
-  =
-    let sf : SF.prog_tree a (M.post_sl_t prd)
-           = lc_sf lc sl0 sl_ro       in
-    let fn : Fun.prog_tree SF2Fun.({val_t = a; sel_t = M.post_sl_t prd})
-           = SF2Fun.repr_Fun_of_SF sf in
-    Fun.tree_wp fn
-
-let lc_wp_sound
-      (#a : Type) (#env : vprop_list) (#t : M.prog_tree a) (#csm : LV.csm_t env) (#prd : LV.prd_t a)
-      (lc : LV.lin_cond u#a u#p env t csm prd)
-      (sl0 : sl_f (lc_pre lc)) (sl_ro : sl_f (lc_ro lc))
-      (post : pure_post SF2Fun.(sl_tys_v ({val_t = a; sel_t = M.post_sl_t prd})))
-  : Lemma (requires lc_wp lc sl0 sl_ro post)
-          (ensures  lc_req lc sl0 sl_ro /\
-                   (forall (x : a) (sl1 : sl_f (prd x)) .
-                    lc_ens lc sl0 x sl1 sl_ro ==> post SF2Fun.({val_v = x; sel_v = sl1})))
-  =
-    let sl0' = LV2SF.append_vars_mask_l csm (Fl.dlist_of_f sl0) (Fl.dlist_of_f sl_ro) in
-    let sf = LV2SF.repr_SF_of_LV lc sl0' in
-    LV2SF.repr_SF_of_LV_sound lc sl0';
-    let fn = SF2Fun.repr_Fun_of_SF sf    in
-    SF2Fun.repr_Fun_of_SF_req sf;
-    Fun.tree_wp_sound fn post;
-    assert (lc_req lc sl0 sl_ro);
-    introduce forall (x : a) (sl1 : sl_f (prd x)) .
-              lc_ens lc sl0 x sl1 sl_ro ==> post SF2Fun.({val_v = x; sel_v = sl1})
-      with SF2Fun.repr_Fun_of_SF_ens sf x sl1
+  | SH.KSteel    -> make_combinator_steel__steel    s f pre_eq post_eq
+  | SH.KAtomic o -> make_combinator_steel__atomic o s f pre_eq post_eq
+  | SH.KGhostI o -> make_combinator_steel__ghostI o s f pre_eq post_eq
+  | SH.KGhost  o -> make_combinator_steel__ghost  o s f pre_eq post_eq
 
 
 (***** [lc_to_spc_steel_t] *)
 
+type lc_repr_steel_t0
+       (#a : Type) (ek : SH.effect_kind) (t : M.prog_tree a)
+       (#env : vprop_list) (#csm : LV.csm_t env) (#prd : LV.prd_t a)
+       (lc : LV.lin_cond u#a u#p env t csm prd {LV.lcsub_at_leaves lc})
+  = M.repr_steel_t ek a env (LV2M.res_env_f env csm prd)
+              (M.tree_req t (LV2M.repr_M_of_LV lc))
+              (M.tree_ens t (LV2M.repr_M_of_LV lc))
+
 #push-options "--fuel 0 --ifuel 0 --z3rlimit 20"
 inline_for_extraction
-let lc_to_spc_steel_t__steel
-      (#a : Type) (mr : M.repr SH.KSteel a)
-      (#env : vprop_list) (#csm : LV.csm_t env) (#prd : LV.prd_t a)
-      (lc : LV.lin_cond u#a u#p env mr.repr_tree csm prd {LV.lcsub_at_leaves lc})
+let lc_to_spc_steel_t_steel__steel
+      (#a : Type) (t : G.erased (M.prog_tree a))
+      (#env : G.erased vprop_list) (#csm : G.erased (LV.csm_t env)) (#prd : G.erased (LV.prd_t a))
+      (lc : G.erased (LV.lin_cond u#a u#p env t csm prd) {LV.lcsub_at_leaves lc})
+      (f : lc_repr_steel_t0 SH.KSteel t lc)
   : M.spc_steel_t SH.KSteel (lc_spec_r lc)
   =
-    let tc = LV2M.repr_M_of_LV lc                              in
-    let sf = mr.repr_steel env (LV2M.res_env_f env csm prd) tc in
+    let tc : G.erased (LV2M.lc_to_M lc) = LV2M.repr_M_of_LV lc in
     (**) LV2M.repr_M_of_LV_sound lc;
     SH.steel_f (fun () ->
       (**) let sl0    = gget_f (lc_pre lc)    in
       (**) let sl_ro0 = gget_f (lc_ro  lc)    in
       elim_vpl_filter_mask_append env csm;
       (**) let sl0'   = gget_f env            in
-      let x = SH.steel_u sf () in
+      let x = SH.steel_u f () in
       (**) let sl1'   = gget_f L.(lc_post lc x @ lc_ro lc) in
       elim_vpl_append (lc_post lc x) (lc_ro lc);
       (**) let sl1    = gget_f (lc_post lc x) in
@@ -322,21 +153,21 @@ let lc_to_spc_steel_t__steel
     )
 
 inline_for_extraction
-let lc_to_spc_steel_t__atomic
-      (opened : Mem.inames) (#a : Type) (mr : M.repr (SH.KAtomic opened) a)
-      (#env : vprop_list) (#csm : LV.csm_t env) (#prd : LV.prd_t a)
-      (lc : LV.lin_cond u#a u#p env mr.repr_tree csm prd {LV.lcsub_at_leaves lc})
+let lc_to_spc_steel_t_steel__atomic
+      (opened : Mem.inames) (#a : Type) (t : G.erased (M.prog_tree a))
+      (#env : G.erased vprop_list) (#csm : G.erased (LV.csm_t env)) (#prd : G.erased (LV.prd_t a))
+      (lc : G.erased (LV.lin_cond u#a u#p env t csm prd) {LV.lcsub_at_leaves lc})
+      (f : lc_repr_steel_t0 (SH.KAtomic opened) t lc)
   : M.spc_steel_t (SH.KAtomic opened) (lc_spec_r lc)
   =
-    let tc = LV2M.repr_M_of_LV lc                              in
-    let sf = mr.repr_steel env (LV2M.res_env_f env csm prd) tc in
+    let tc : G.erased (LV2M.lc_to_M lc) = LV2M.repr_M_of_LV lc in
     (**) LV2M.repr_M_of_LV_sound lc;
     SH.atomic_f #opened (fun () ->
       (**) let sl0    = gget_f (lc_pre lc)    in
       (**) let sl_ro0 = gget_f (lc_ro  lc)    in
       elim_vpl_filter_mask_append env csm;
       (**) let sl0'   = gget_f env            in
-      let x = SH.atomic_u sf () in
+      let x = SH.atomic_u f () in
       (**) let sl1'   = gget_f L.(lc_post lc x @ lc_ro lc) in
       elim_vpl_append (lc_post lc x) (lc_ro lc);
       (**) let sl1    = gget_f (lc_post lc x) in
@@ -349,21 +180,48 @@ let lc_to_spc_steel_t__atomic
     )
 
 inline_for_extraction
-let lc_to_spc_steel_t__ghost
-      (opened : Mem.inames) (#a : Type) (mr : M.repr (SH.KGhost opened) a)
-      (#env : vprop_list) (#csm : LV.csm_t env) (#prd : LV.prd_t a)
-      (lc : LV.lin_cond u#a u#p env mr.repr_tree csm prd {LV.lcsub_at_leaves lc})
+let lc_to_spc_steel_t_steel__ghostI
+      (opened : Mem.inames) (#a : Type) (t : G.erased (M.prog_tree a))
+      (#env : G.erased vprop_list) (#csm : G.erased (LV.csm_t env)) (#prd : G.erased (LV.prd_t a))
+      (lc : G.erased (LV.lin_cond u#a u#p env t csm prd) {LV.lcsub_at_leaves lc})
+      (f : lc_repr_steel_t0 (SH.KGhostI opened) t lc)
+  : M.spc_steel_t (SH.KGhostI opened) (lc_spec_r lc)
+  =
+    let tc : G.erased (LV2M.lc_to_M lc) = LV2M.repr_M_of_LV lc in
+    (**) LV2M.repr_M_of_LV_sound lc;
+    SH.ghostI_f #opened (fun () ->
+      (**) let sl0    = gget_f (lc_pre lc)    in
+      (**) let sl_ro0 = gget_f (lc_ro  lc)    in
+      elim_vpl_filter_mask_append env csm;
+      (**) let sl0'   = gget_f env            in
+      let x = SH.ghostI_u f () in
+      (**) let sl1'   = gget_f L.(lc_post lc x @ lc_ro lc) in
+      elim_vpl_append (lc_post lc x) (lc_ro lc);
+      (**) let sl1    = gget_f (lc_post lc x) in
+      (**) let sl_ro1 = gget_f (lc_ro   lc)   in
+      (**) assert (Ghost.reveal sl1' == LV2M.res_env_app sl1 sl_ro1);
+      (**) assert (M.tree_ens _ tc sl0' x sl1');
+      (**) filter_append_vars_mask csm sl0 sl_ro0;
+      (**) assert (LV.tree_ens lc sl0' x sl1 /\ sl_ro0 == sl_ro1);
+      SA.return x
+    )
+
+inline_for_extraction
+let lc_to_spc_steel_t_steel__ghost
+      (opened : Mem.inames) (#a : Type) (t : G.erased (M.prog_tree a))
+      (#env : G.erased vprop_list) (#csm : G.erased (LV.csm_t env)) (#prd : G.erased (LV.prd_t a))
+      (lc : G.erased (LV.lin_cond u#a u#p env t csm prd) {LV.lcsub_at_leaves lc})
+      (f : lc_repr_steel_t0 (SH.KGhost opened) t lc)
   : M.spc_steel_t (SH.KGhost opened) (lc_spec_r lc)
   =
-    let tc = LV2M.repr_M_of_LV lc                              in
-    let sf = mr.repr_steel env (LV2M.res_env_f env csm prd) tc in
+    let tc : G.erased (LV2M.lc_to_M lc) = LV2M.repr_M_of_LV lc in
     (**) LV2M.repr_M_of_LV_sound lc;
     SH.ghost_f #opened (fun () ->
       (**) let sl0    = gget_f (lc_pre lc)    in
       (**) let sl_ro0 = gget_f (lc_ro  lc)    in
       elim_vpl_filter_mask_append env csm;
       (**) let sl0'   = gget_f env            in
-      let x = SH.ghost_u sf () in
+      let x = SH.ghost_u f () in
       (**) let sl1'   = gget_f L.(lc_post lc x @ lc_ro lc) in
       elim_vpl_append (lc_post lc x) (lc_ro lc);
       (**) let sl1    = gget_f (lc_post lc x) in
@@ -375,339 +233,17 @@ let lc_to_spc_steel_t__ghost
       (**) noop ();
       x
     )
-
-inline_for_extraction
-let lc_to_spc_steel_t__ghostI
-      (opened : Mem.inames) (#a : Type) (mr : M.repr (SH.KGhostI opened) a)
-      (#env : vprop_list) (#csm : LV.csm_t env) (#prd : LV.prd_t a)
-      (lc : LV.lin_cond u#a u#p env mr.repr_tree csm prd {LV.lcsub_at_leaves lc})
-  : M.spc_steel_t (SH.KGhostI opened) (lc_spec_r lc)
-  =
-    let tc = LV2M.repr_M_of_LV lc                              in
-    let sf = mr.repr_steel env (LV2M.res_env_f env csm prd) tc in
-    (**) LV2M.repr_M_of_LV_sound lc;
-    SH.ghostI_f #opened (fun () ->
-      (**) let sl0    = gget_f (lc_pre lc)    in
-      (**) let sl_ro0 = gget_f (lc_ro  lc)    in
-      elim_vpl_filter_mask_append env csm;
-      (**) let sl0'   = gget_f env            in
-      let x = SH.ghostI_u sf () in
-      (**) let sl1'   = gget_f L.(lc_post lc x @ lc_ro lc) in
-      elim_vpl_append (lc_post lc x) (lc_ro lc);
-      (**) let sl1    = gget_f (lc_post lc x) in
-      (**) let sl_ro1 = gget_f (lc_ro   lc)   in
-      (**) assert (Ghost.reveal sl1' == LV2M.res_env_app sl1 sl_ro1);
-      (**) assert (M.tree_ens _ tc sl0' x sl1');
-      (**) filter_append_vars_mask csm sl0 sl_ro0;
-      (**) assert (LV.tree_ens lc sl0' x sl1 /\ sl_ro0 == sl_ro1);
-      SA.return x
-    )
 #pop-options
 
 inline_for_extraction
-let lc_to_spc_steel_t
-      (#ek : SH.effect_kind) (#a : Type) (mr : M.repr ek a)
-      (#env : vprop_list) (#csm : LV.csm_t env) (#prd : LV.prd_t a)
-      (lc : LV.lin_cond u#a u#p env mr.repr_tree csm prd {LV.lcsub_at_leaves lc})
+let lc_to_spc_steel_t_steel
+      (#ek : SH.effect_kind) (#a : Type) (t : G.erased (M.prog_tree a))
+      (#env : G.erased vprop_list) (#csm : G.erased (LV.csm_t env)) (#prd : G.erased (LV.prd_t a))
+      (lc : G.erased (LV.lin_cond u#a u#p env t csm prd) {LV.lcsub_at_leaves lc})
+      (f : lc_repr_steel_t0 ek t lc)
   : M.spc_steel_t ek (lc_spec_r lc)
-  =
-    match ek with
-    | SH.KSteel    -> lc_to_spc_steel_t__steel    mr lc
-    | SH.KAtomic o -> lc_to_spc_steel_t__atomic o mr lc
-    | SH.KGhost  o -> lc_to_spc_steel_t__ghost  o mr lc
-    | SH.KGhostI o -> lc_to_spc_steel_t__ghostI o mr lc
-
-
-(*** Building [lin_cond] *)
-
-(**** Enforcing [lcsub_at_leaves] *)
-
-[@@ __cond_solver__]
-let build_lcsub_at_leaves_lc
-       (env : vprop_list) (#a : Type) (t : M.prog_tree a)
-       (csm : LV.csm_t env) (prd : LV.prd_t a)
-       (lc0 : LV.lin_cond u#a u#p env #a t csm prd)
-  : lc : LV.lin_cond env #a t csm prd { LV.lcsub_at_leaves lc }
-  =
-    (**) LV.lc_sub_push_at_leaves env lc0;
-    LV.lc_sub_push lc0
-
-
-(**** With exact specifications *)
-
-[@@ __cond_solver__]
-let __build_lin_cond_exact
-      (env : vprop_list) (#a : Type) (t : M.prog_tree a)
-      (csm0 csm1 : LV.csm_t env) (prd0 prd1 : LV.prd_t a)
-      (lc : LV.lin_cond env t csm0 prd0)
-      (csm_le : b2t (Msk.mask_le_eff csm0 csm1))
-      (prd_f : (x : a) -> Perm.pequiv_list L.(prd0 x @ filter_diff csm0 csm1 env) (prd1 x))
-  : LV.lin_cond env t csm1 prd1
-  =
-    Ll.list_extensionality (Msk.mask_or csm0 csm1) csm1 (fun i -> ());
-    lcsub_add_csm env t csm0 prd0 lc csm1 prd1 prd_f
-
-/// Solves a goal [lin_cond env t prd csm] where [prd] and [csm] are concrete terms.
-let build_lin_cond_exact (fr : flags_record) (ctx : cs_context) : Tac unit
-  =
-    apply (`__build_lin_cond_exact);
-    // lc
-    build_lin_cond fr ctx None;
-    // csm_le
-    norm_lc ();
-    cs_try (fun () ->
-        norm [delta_only [`%Msk.mask_le_eff]; iota; zeta; primops];
-        trefl ()
-      ) fr ctx (fun m -> fail (m Fail_csm_le []));
-    // prd_f
-    let x = intro () in
-    norm_lc ();
-    build_pequiv_list fr ctx
-
-#push-options "--fuel 5"
-let test_lin_cond_exact (v : int -> vprop')
-  : LV.lin_cond [v 0; v 1; v 2]
-      M.(Tspec unit (M.spec_r_exact (Mkspec_r [v 0] (fun _ -> [v 3]) [v 1] (fun _ _ -> True) (fun _ _ _ _ -> True))))
-      [true; false; true] (fun _ -> [v 2; v 3])
-  = _ by (build_lin_cond_exact default_flags dummy_ctx)
-#pop-options
-
-
-(**** [lin_cond_st] *)
-
-/// [lin_cond_st env t must_csm must_prd csm1 prd1] ("lin_cond such that") is used to build a [lin_cond] consuming at
-/// least [must_csm] and producing at least [must_prd]. It allows other variables to be consumed ([csm1]) or
-/// produced ([prd1]).
-
-#push-options "--ifuel 0 --fuel 0"
-
-type lin_cond_st
-       (env : vprop_list) (#a : Type) (t : M.prog_tree a)
-       (must_csm : LV.csm_t env) (must_prd : LV.prd_t a)
-       (csm1 : LV.csm_t Msk.(filter_mask (mask_not must_csm) env)) (prd1 : LV.prd_t a)
-  = lc : LV.lin_cond u#a u#p env #a t (Msk.mask_comp_or must_csm csm1) L.(fun x -> must_prd x @ prd1 x)
-       { LV.lcsub_at_leaves lc }
-
-let pequiv_append_02 (#a : Type) (l0 l1 l2 l3 : list a)
-  : Perm.pequiv L.(l0 @ l1 @ l2 @ l3) L.(l0 @ l2 @ l1 @ l3)
-  =
-    L.append_assoc l1 l2 l3; L.append_assoc l2 l1 l3;
-    U.cast _
-    Perm.(pequiv_append (pequiv_refl l0)
-         (pequiv_append (pequiv_append_swap l1 l2)
-                        (pequiv_refl l3)))
-
-[@@ __cond_solver__]
-let build_lin_cond_st_prd_f
-      (prd0 env must_prd : vprop_list) (must_csm : LV.csm_t env)
-      (post_f : LV.eq_injection_l must_prd L.(prd0 @ env))
-  : (let n0 = L.length prd0          in
-     let n1 = L.length env           in
-     let m0 = LV.eij_trg_mask post_f in
-     (**) L.splitAt_length n0 m0;
-     let m0a, m0b = L.splitAt n0 m0  in
-     let m0a : Ll.vec n0 bool = m0a  in
-     let m0b : Ll.vec n1 bool = m0b  in
-     Perm.pequiv_list
-      L.(prd0 @ Msk.(filter_mask (mask_or m0b must_csm) env))
-      L.(must_prd @ Msk.(filter_mask (mask_not m0a) prd0) @ filter_diff m0b must_csm env))
-  = Msk.(
-    let n0 = L.length prd0          in
-    let n1 = L.length env           in
-    let m0 = LV.eij_trg_mask post_f in
-    (**) L.splitAt_length n0 m0;
-    let m0a, m0b = L.splitAt n0 m0  in
-    let m0a : Ll.vec n0 bool = m0a  in
-    let m0b : Ll.vec n1 bool = m0b  in
-
-    let must_csm' = mask_diff m0b must_csm in
-
-    let flt00 = filter_mask m0a prd0                                   in
-    let flt01 = filter_mask (mask_not m0a) prd0                        in
-    let flt10 = filter_mask m0b env                                    in
-    let flt11 = filter_mask must_csm' (filter_mask (mask_not m0b) env) in
-
-    Ll.list_extensionality (mask_or m0b must_csm) (mask_comp_or m0b must_csm') (fun i -> ());
-    assert (filter_diff m0b must_csm env == flt11);
-    U.assert_by L.(filter_mask m0 (prd0 @ env) == flt00 @ flt10) (fun () ->
-      Ll.lemma_splitAt_append n0 m0;
-      filter_mask_append m0a m0b prd0 env);
-
-    let f0 : Perm.pequiv L.(flt00 @ flt10) must_prd
-      = U.cast _ (LV.eij_equiv post_f)           in
-    let f1 : Perm.pequiv prd0 L.(flt00 @ flt01)
-      = mask_pequiv_append m0a prd0              in
-    let f2 : Perm.pequiv (filter_mask (mask_comp_or m0b must_csm') env) L.(flt10 @ flt11)
-      = mask_or_pequiv_append m0b must_csm' env  in
-
-    L.append_assoc flt00 flt01 L.(flt10 @ flt11);
-    let f3 : Perm.pequiv L.(prd0 @ filter_mask (mask_comp_or m0b must_csm') env)
-                         L.(flt00 @ flt01 @ flt10 @ flt11)
-      = Perm.pequiv_append f1 f2                 in
-    L.append_assoc flt00 flt10 L.(flt01 @ flt11);
-    let f4 : Perm.pequiv L.(flt00 @ flt01 @ flt10 @ flt11)
-                         L.((flt00 @ flt10) @ (flt01 @ flt11))
-      = pequiv_append_02 flt00 flt01 flt10 flt11 in
-
-    let f : Perm.pequiv L.(prd0 @ filter_mask (mask_comp_or m0b must_csm') env)
-                        L.(must_prd @ (flt01 @ flt11))
-      = Perm.(pequiv_trans f3
-             (pequiv_trans f4
-             (pequiv_append f0 (pequiv_refl L.(flt01 @ flt11)))))
-    in Perm.perm_f_to_list f)
-
-[@@ __cond_solver__]
-let __build_lin_cond_st
-      (env : vprop_list) (#a : Type) (t : M.prog_tree a)
-      (csm0 : LV.csm_t env) (prd0 : LV.prd_t a)
-      (ct : LV.lin_cond env t csm0 prd0)
-      (must_csm : LV.csm_t env) (must_prd : LV.prd_t a)
-      (post_f : (x : a) -> LV.eq_injection_l (must_prd x) (LV.res_env env csm0 (prd0 x)))
-      (csm' : Msk.(mask_t (filter_mask (mask_not csm0) env)))
-      (csm'_eq : (x : a) -> squash (
-        let n0 = L.length (prd0 x)          in
-        let m0 = LV.eij_trg_mask (post_f x) in
-        (**) L.splitAt_length n0 m0;
-        csm' = (L.splitAt n0 m0)._2))
-  : lin_cond_st u#a u#p env t must_csm must_prd
-        Msk.(mask_diff must_csm (mask_comp_or csm0 csm'))
-        (fun x ->
-          let n0 = L.length (prd0 x)          in
-          let m0 = LV.eij_trg_mask (post_f x) in
-          (**) L.splitAt_length n0 m0;
-          let m0a : Ll.vec n0 bool = (L.splitAt n0 m0)._1 in
-          L.(Msk.filter_mask (Msk.mask_not m0a) (prd0 x)
-           @ filter_diff (Msk.mask_comp_or csm0 csm') must_csm env))
-  =
-    let csm1 : Msk.(mask_t (filter_mask (mask_not csm0) env))
-             = Msk.(mask_or csm' (mask_diff csm0 must_csm))     in
-    let prd1 x =
-      let n0 = L.length (prd0 x)                                in
-      let m0 = LV.eij_trg_mask (post_f x)                       in
-      (**) L.splitAt_length n0 m0;
-      let m0a : Ll.vec n0 bool = (L.splitAt n0 m0)._1           in
-      L.(Msk.filter_mask (Msk.mask_not m0a) (prd0 x)
-       @ filter_diff (Msk.mask_comp_or csm0 csm') must_csm env) in
-    Msk.(calc (==) {
-      LV.bind_csm env csm0 csm1 <: list bool;
-    == { Ll.list_extensionality_sq (fun i -> ()) }
-      mask_or must_csm (mask_comp_or csm0 csm');
-    == { mask_comp_or_mask_diff must_csm (mask_comp_or csm0 csm') }
-      mask_comp_or must_csm (mask_diff must_csm (mask_comp_or csm0 csm'));
-    });
-    let prd_f (x : a) : Perm.pequiv_list (LV.sub_prd env csm0 (prd0 x) csm1) L.(must_prd x @ prd1 x)
-      =
-        let n0 = L.length (prd0 x)              in
-        let n1 = Msk.(mask_len (mask_not csm0)) in
-        let m0 = LV.eij_trg_mask (post_f x)     in
-        (**) L.splitAt_length n0 m0;
-        let m0a, m0b = L.splitAt n0 m0          in
-        let m0a : Ll.vec n0 bool = m0a          in
-        let m0b : Ll.vec n1 bool = m0b          in
-        U.assert_by (csm' == m0b) (fun () -> csm'_eq x);
-        let env1      = Msk.(filter_mask (mask_not csm0) env) in
-        let must_csm1 = Msk.(mask_diff csm0 must_csm)         in
-        assert (LV.sub_prd env csm0 (prd0 x) csm1
-          == L.(prd0 x @ Msk.(filter_mask (mask_or m0b must_csm1) env1)));
-        Msk.(calc (==) {
-          filter_diff m0b (mask_diff csm0 must_csm) (filter_mask (mask_not csm0) env);
-        == { }
-          filter_mask (mask_diff m0b (mask_diff csm0 must_csm))
-            (filter_mask (mask_not m0b) (filter_mask (mask_not csm0) env));
-        == { filter_mask_and (mask_not csm0) (mask_not m0b) must_csm;
-             filter_mask_and (mask_not csm0) (mask_not m0b) env }
-          filter_mask (filter_mask (mask_comp_and (mask_not csm0) (mask_not m0b)) must_csm)
-            (filter_mask (mask_comp_and (mask_not csm0) (mask_not m0b)) env);
-        == { mask_not_comp_or csm0 m0b }
-          filter_mask (filter_mask (mask_not (mask_comp_or csm0 m0b)) must_csm)
-            (filter_mask (mask_not (mask_comp_or csm0 m0b)) env);
-        == { }
-          filter_diff (mask_comp_or csm0 m0b) must_csm env;
-        });
-        assert L.(must_prd x @ prd1 x
-               == must_prd x @ Msk.(filter_mask (mask_not m0a) (prd0 x)) @ filter_diff m0b must_csm1 env1);
-        build_lin_cond_st_prd_f (prd0 x) env1 (must_prd x) must_csm1 (post_f x)
-    in
-    let ct' = LV.LCsub env csm0 prd0 ct csm1 L.(fun x -> must_prd x @ prd1 x) prd_f in
-    (**) LV.lc_sub_push_at_leaves env ct';
-    LV.lc_sub_push ct'
-
-
-noeq
-type test_lin_cond_st env #a t must_csm must_prd =
-  | TestLinCondSt : (csm1 : _) -> (prd1 : _) ->
-                    lin_cond_st env #a t must_csm must_prd csm1 prd1 ->
-                    test_lin_cond_st env t must_csm must_prd
-
-#push-options "--fuel 5"
-let test_lin_cond_st_0 (v : int -> vprop')
-  : test_lin_cond_st [v 0; v 1; v 2; v 3]
-      M.(Tspec unit (M.spec_r_exact (Mkspec_r [v 0] (fun _ -> [v 4; v 5]) [v 1] (fun _ _ -> True) (fun _ _ _ _ -> True))))
-      [true; false; true; false] (fun _ -> [v 4; v 1])
-  = _ by (
-    apply (`TestLinCondSt);
-    apply_raw (`__build_lin_cond_st);
-    // ct
-    dismiss (); dismiss ();
-    build_lin_cond default_flags dummy_ctx None;
-    // post_f
-    let x = intro () in
-    norm_lc ();
-    build_eq_injection_l default_flags dummy_ctx;
-    // csm'_eq
-    dismiss ();
-    let x = intro () in
-    norm_lc ();
-    trefl ()
-  )
-#pop-options
-
-[@@ __cond_solver__]
-let __normalize_lin_cond_st
-       (env : vprop_list) (#a : Type) (t : M.prog_tree a)
-       (must_csm : LV.csm_t env) (must_prd : LV.prd_t a)
-       (csm1 : LV.csm_t Msk.(filter_mask (mask_not must_csm) env)) (prd1 : LV.prd_t a)
-       (lc : lin_cond_st env t must_csm must_prd csm1 prd1)
-       (lc1 : lin_cond_st env t must_csm must_prd csm1 prd1)
-       (_ : squash (lc1 == lc))
-       (csm2 : LV.csm_t Msk.(filter_mask (mask_not must_csm) env)) (prd2 : LV.prd_t a)
-       (_ : squash (csm2 == csm1 /\ prd2 == prd1))
-  : lin_cond_st u#a u#p env t must_csm must_prd csm2 prd2
-  = lc1
-
-#pop-options
-
-#push-options "--ifuel 1"
-/// Solves a goal [lin_cond_st env t must_csm must_prd ?csm1 ?prd1]
-let build_lin_cond_st (fr : flags_record) (ctx : cs_context) : Tac unit
-  =
-    apply_raw (`__normalize_lin_cond_st);
-    // lc
-      dismiss (); dismiss ();
-      apply_raw (`__build_lin_cond_st);
-      // ct
-      dismiss (); dismiss ();
-      build_lin_cond fr ctx None;
-      // post_f
-      let x = intro () in
-      norm_lc ();
-      build_eq_injection_l fr ctx;
-      // csm'_eq
-      dismiss ();
-      let x = intro () in
-      norm_lc ();
-      cs_try trefl fr ctx (fun m -> fail (m (Fail_dependency "csm" x) []));
-    // lc1 <-
-    dismiss ();
-    norm [
-      delta_only (L.append __delta_list (L.append __delta_perm [
-        `%L.splitAt; `%L.mem; `%Mktuple2?._1; `%Mktuple2?._2; `%L.map2;
-        `%pequiv_append_02]));
-      delta_attr [`%__cond_solver__; `%Learn.Tactics.Util.__tac_helper__; `%Msk.__mask__; `%LV.__lin_cond__];
-      delta_qualifier ["unfold"];
-      iota; zeta; primops];
-    trefl ();
-    // csm2, prd2 <-
-    norm_lc ();
-    split (); trefl (); trefl ()
-#pop-options
+  = match ek with
+    | SH.KSteel    -> lc_to_spc_steel_t_steel__steel    t lc f
+    | SH.KAtomic o -> lc_to_spc_steel_t_steel__atomic o t lc f
+    | SH.KGhost  o -> lc_to_spc_steel_t_steel__ghost  o t lc f
+    | SH.KGhostI o -> lc_to_spc_steel_t_steel__ghostI o t lc f
